Add files via upload

Treiber Stack C11/RCU.thy
@@ -1,1041 +1,281 @@
 theory RCU
-imports Main PSem
+imports RCU_model
 begin 
 
+(*the following must be included in the proof:
 
+con_assms ps        --- concerns allocation/bounds of C and rcu_0+i for all i
+main_inv ms             --- main invariant has 3 parts
 
-datatype PC = I1 | I2 | I3 | I4 | I5 | I6 | I7 | I8 | I9 | I10 | I11 | I12 | I13 | I14 |  cas_res | finished
-            | R1 | R2 | R3 | R4 | R5 
-            | S1 | S2 | S3 | S4 | S5 | S6 | S7 
+nts::
+psem_rules ps               --- how allocation works on the inside
 
+tedious - general_structure ms                      --- says how n \<noteq> s \<noteq> detaddrs
+allocated_addresses ms ps *********        --- allocation for above are defined here
+simple - observation_inv_ms ms         --- how own\<^sub>W affects loc status (own\<^sub>W loc = t \<longrightarrow> loc\<in>{s,n,det} t)
+hard - observation_inv_sig ms ps \<sigma>       --- limits which values can be WM_read from C
+simple - own\<^sub>W_n_by_t_imp ms
 
 
-consts rcu_0 ::address (*first location of rcu array*)
-consts F::nat
-consts T_max::nat (*max_thread ID - 1*)
-consts C :: nat     (*just referred to by its location in A(1) = (C,pointer) where C = nat*)
-consts casloc :: nat
-definition "set_T \<equiv> {n . n\<ge>0 \<and> n<T_max}"
-definition "rcu_addrs \<equiv> {n . n\<ge>rcu_0 \<and> n < rcu_0+T_max}"
-definition "something  \<equiv> F \<notin> rcu_addrs \<and> F \<noteq> C \<and> F \<noteq> casloc"
+t \<le> T_max
+step ms ps \<sigma> (pc ms t) t ms' ps' \<sigma>'     --- defines a program step by t
+last - preCond ms ps \<sigma> (pc ms t) t             --- defines preconditions for t to proceed with stepping      
 
 
 
-lemma test:
-  assumes "F = i"
-  and "something"
-  shows "C \<noteq> i"
-  using assms 
-  by(simp add:something_def) 
 
-
-
-
-
-
-(*Recorded variables partial function*)
-record mstate =
-  pc :: "T \<Rightarrow> PC"
-  r :: "T \<Rightarrow> nat \<Rightarrow> nat"        (*local copy of rcu*)
-  n_dec :: "T \<Rightarrow> bool"        (*now modelled as local pointer allocation - True/False*)
-  s_dec :: "T \<Rightarrow> bool"        (*now modelled as local pointer allocation - True/False*)
-  v :: "T \<Rightarrow> nat option"        (*now modelled as local value - so M(&v)*)
-  n :: "T \<Rightarrow> nat option"        (*now modelled as local value - so M(&n)*)
-  s :: "T \<Rightarrow> nat option"        (*now modelled as local value - so M(&s)*)
-  det :: "T \<Rightarrow> L list"   (*detached list*)
-  CTRsync\<^sub>1 :: "T \<Rightarrow> nat"
-  CTRsync\<^sub>2 :: "T \<Rightarrow> nat"
-  res :: "T \<Rightarrow> nat"           (*return v*)
-  reg :: "T \<Rightarrow> nat"            (*says whether a thread is locally in RCU or not*)
-  nondet_val :: "T \<Rightarrow> bool"    (* result of function nondet() *)
-  CAS_succ :: "T \<Rightarrow> bool"      (*CAS succ, aux*)
-  repeat :: "T \<Rightarrow> bool"              (*says whether the CAS has failed*)
-
-  own\<^sub>R :: "nat \<Rightarrow> nat set"      (* own\<^sub>R ms i = { ... 2, 3, 6, ...}*)
-  own\<^sub>W :: "nat \<Rightarrow> nat option"   (* own\<^sub>W ms i = Some 1 or own\<^sub>W ms i = None*)
-
-
-(*for pointers we will have A(0) = (x58,pointer) which is equivalent to   A(order) = (address,pointer)
-  for variables  --//---    A(1) = (x78,variable) --//--    --//--        A(order) = (address,variable)*)
-  
-
-(* start state must take out rcu_addrs  from free_addrs *)
-
-(*---------------- ownership transfer functions ---------------------*)
-
-definition take_read_ownership :: "T \<Rightarrow> nat \<Rightarrow> mstate \<Rightarrow> mstate" ("takesRown[_,_]" [200,200])
-  where
-  "take_read_ownership t loc ms \<equiv>  ms \<lparr> own\<^sub>R := (own\<^sub>R ms) (loc:=own\<^sub>R ms loc \<union> {t}) \<rparr>"
-
-definition giveup_readandwrite_ownership :: "T \<Rightarrow> nat \<Rightarrow> mstate \<Rightarrow> mstate" ("givesupRown[_,_]" [200,200])
-  where
-  "giveup_readandwrite_ownership t loc ms \<equiv>  ms \<lparr> own\<^sub>R := (own\<^sub>R ms) (loc:=own\<^sub>R ms loc - {t}) \<rparr>"
-
-definition take_write_ownership :: "T \<Rightarrow> nat \<Rightarrow> mstate \<Rightarrow> mstate" ("takesWown[_,_]" [200,200])
-  where
-  "take_write_ownership t loc ms \<equiv>   ms \<lparr> own\<^sub>R := (own\<^sub>R ms) (loc:=own\<^sub>R ms loc \<union> {t}),
-                                          own\<^sub>W := (own\<^sub>W ms) (loc:=Some t)\<rparr>"
-
-
-
-
-(*---------------- basic functional definitons ----------------------*)
-
-(*int v*)
-definition v_allocation :: "mstate \<Rightarrow> T \<Rightarrow> mstate \<Rightarrow> bool" ("_ int[v\<^sub>_] _" [200,200])           \<comment>\<open>int v, note v is a local variable\<close>
-  where                                                                                           \<comment>\<open>  and doesn't need allocation\<close>
-  "v_allocation ms t ms' \<equiv>  ms' =ms \<lparr>v := (v ms) (t := None),
-                                    pc := (pc ms) (t := I2)\<rparr>"
-(*int *n*)
-definition int_star_n :: "mstate \<Rightarrow> T \<Rightarrow> mstate \<Rightarrow> bool" ("_ int[*n\<^sub>_] _" [200,200,200])           \<comment>\<open>int *n\<close>
-  where
-  "int_star_n ms t ms' \<equiv> ms' = ms \<lparr>n_dec := (n_dec ms) (t := True),
-                               n := (n ms) (t := None),
-                                  pc := (pc ms) (t := I3)\<rparr>"
-(*int *s*)
-definition int_star_s :: "mstate \<Rightarrow> T \<Rightarrow> mstate \<Rightarrow> bool" ("_ int[*s\<^sub>_] _" [200,200,200])           \<comment>\<open>int *s\<close>
-  where
-  "int_star_s ms t ms' \<equiv> ms' = ms \<lparr>s_dec := (s_dec ms) (t := True),
-                               s := (s ms) (t := None),
-                                  pc := (pc ms) (t := I4) \<rparr>"
-
-
-
-
-(*******   n = new int  **********)
-definition new_int :: "mstate \<Rightarrow> posem \<Rightarrow> T \<Rightarrow> mstate \<Rightarrow> posem \<Rightarrow> bool" ( "_ _ n:=newint _ _ _" [200,200,200,200,200])
-  where
-  "new_int ms ps t ms' ps' \<equiv>  (\<exists>loc prov. (allocate_object ps loc prov ps' variable 
-                                    \<and> ms' = ms \<lparr>n := (n ms) (t := Some loc),
-                                                 own\<^sub>R := (own\<^sub>R ms) (loc:=own\<^sub>R ms loc \<union> {t}),
-                                                 own\<^sub>W := (own\<^sub>W ms) (loc:=Some t),
-                                                   pc := (pc ms) (t := I5) \<rparr>))"
-
-lemma switch:
-  "prov\<notin> dom(A ps) \<longrightarrow> A ps prov = None"
-  by auto
-
-lemma switch2:
-  "n ms t = None \<Longrightarrow> \<exists>prov loc. (allocate_object ps loc prov ps' variable  
-                                    \<and> ms' = ms \<lparr>n := (n ms) (t := Some loc),
-                                             own\<^sub>R := (own\<^sub>R ms) (loc:=own\<^sub>R ms loc \<union> {t}),
-                                             own\<^sub>W := (own\<^sub>W ms) (loc:=Some t),
-                                               pc := (pc ms) (t := I5) \<rparr>) 
-      \<Longrightarrow> n ms' t\<noteq> None"
-  apply(simp add:new_int_def) apply clarify
-  by simp
-
-lemma switch3:
-  "n ms t = None \<Longrightarrow> \<exists>prov loc. (allocate_object ps loc prov ps' variable  
-                                    \<and> ms' = ms \<lparr>n := (n ms) (t := Some loc),
-                                             own\<^sub>R := (own\<^sub>R ms) (loc:=own\<^sub>R ms loc \<union> {t}),
-                                             own\<^sub>W := (own\<^sub>W ms) (loc:=Some t),
-                                               pc := (pc ms) (t := I5) \<rparr>) 
-    \<Longrightarrow> own\<^sub>W ms' (the(n ms' t)) =Some  t"
-  apply(simp add:new_int_def) apply clarify 
-  by clarsimp
-
-
-
-
-
-
-
-
-
-(*******   s = C   **********)
-definition get_C_val :: "mstate \<Rightarrow> surrey_state \<Rightarrow> T \<Rightarrow> mstate \<Rightarrow> surrey_state \<Rightarrow> bool" ( "_ _ s:=\<^sup>FC _ _ _" [200,200,200,200,200])
-  where
-  "get_C_val ms \<sigma> t ms' \<sigma>' \<equiv> (\<exists> w ts'.
-                                      w \<in> visible_writes \<sigma> t C \<and>
-                                      w \<notin> covered \<sigma> \<and>
-                                      valid_fresh_ts \<sigma> w ts' \<and>
-              \<sigma>' = fst(FAAZ t w \<sigma> ts')
-           \<and> ms' = ms \<lparr> s := (s ms) (t := Some (snd(FAAZ t w \<sigma> ts'))),
-                       pc := (pc ms) (t := I9),
-                     own\<^sub>R := (own\<^sub>R ms) ((snd(FAAZ t w \<sigma> ts')):=own\<^sub>R ms (snd(FAAZ t w \<sigma> ts')) \<union> {t})\<rparr>)" 
-
-
-
-
-
-
-
-(*******   v=*s   **********)
-definition get_s :: "mstate \<Rightarrow> surrey_state \<Rightarrow> T  \<Rightarrow> mstate \<Rightarrow> surrey_state \<Rightarrow> bool" ( "_ _ v:=*s _ _ _" [200,200,200,200,200])
-  where
-  "get_s ms \<sigma> t ms' \<sigma>' \<equiv>  (\<exists>z.  \<sigma> [z \<leftarrow> the (s ms t)]\<^sub>t \<sigma>'
-                                      \<and> ms' = ms \<lparr> v := (v ms) (t := Some z),
-                                                      pc := (pc ms) (t := I10)\<rparr>)" 
-
-
-(*******   *n = v+1   **********) 
-definition writeto_star_n :: "mstate \<Rightarrow> surrey_state \<Rightarrow> T  \<Rightarrow> mstate \<Rightarrow> surrey_state \<Rightarrow> bool" ( "_ _ *n:=newv _ _ _" [200,200,200,200,200])
-  where
-  "writeto_star_n ms \<sigma> t ms' \<sigma>' \<equiv>  \<sigma> [the(n ms t) := (the (v ms t) + 1)]\<^sub>t \<sigma>'
-                                          \<and>  ms' = ms \<lparr>pc := (pc ms) (t := I11)\<rparr>"   
-
-
-
-
-
-
-
-(********* free(pop(detached)) ******************)
-definition pop_address :: "mstate \<Rightarrow> posem \<Rightarrow> T \<Rightarrow> mstate \<Rightarrow> posem \<Rightarrow> bool" ("_ _ free[pop[detached[_]]] _ _" [200,200,200,200,200])    \<comment>\<open>pop(detached[tid-1])\<close>
-  where
-  "pop_address ms ps t ms' ps' \<equiv> (\<exists>i. (A ps i = Some (hd((det ms) t), variable) \<and>
-                                       kill ps i ps')) \<and> 
-                        ms' = ms\<lparr> det := (det ms) (t:= tl ((det ms) t)),
-                                 own\<^sub>R := (own\<^sub>R ms) ((hd((det ms) t)):=(own\<^sub>R ms (hd((det ms) t))) - {t}),
-                                 own\<^sub>W := (own\<^sub>W ms) ((hd((det ms) t)):=None),
-                                  pc := (pc ms) (t := R4)\<rparr> "
-
-
-
-(*******   r[i] = rcu[i]   **********)
-definition load_rcu_to_r :: "mstate \<Rightarrow> posem \<Rightarrow> surrey_state \<Rightarrow>  T \<Rightarrow> mstate \<Rightarrow> posem \<Rightarrow> surrey_state \<Rightarrow> bool" ( "_ _ _ r[i]:=rcu[i] _ _ _ _" [200,200,200,200,200])
-  where
-  "load_rcu_to_r ms ps \<sigma> t ms' ps' \<sigma>' \<equiv> ps = ps' \<and> (\<exists>x y.  (A ps y = Some (rcu_0, pointer)) 
-                                      \<and> \<sigma> [x \<leftarrow>(rcu_0 + (CTRsync\<^sub>1 ms t))]\<^sub>t \<sigma>'
-                                      \<and> ms' = ms \<lparr> r := (r ms) (t := ((r ms) t) ((CTRsync\<^sub>1 ms t) :=x)),
-                                                  pc := (pc ms) (t := S2) \<rparr>)"
-
-definition enter_rcu :: "posem \<Rightarrow> surrey_state \<Rightarrow> T \<Rightarrow> posem \<Rightarrow> surrey_state \<Rightarrow> bool" ( "_ _ rcuenter[] _ _ _" [200,200,200,200,200])
-  where
-  "enter_rcu ps \<sigma> t  ps' \<sigma>' \<equiv>  ps = ps' \<and> (\<exists>x.  (A ps x = Some (rcu_0, pointer))
-                                      \<and> (\<sigma> [ (rcu_0+t) := 1 ]\<^sub>t \<sigma>'))" 
-
-definition exit_rcu :: "posem \<Rightarrow> surrey_state \<Rightarrow> T \<Rightarrow> posem \<Rightarrow> surrey_state \<Rightarrow> bool" ( "_ _ rcuexit[] _ _ _" [200,200,200,200,200])
-  where
-  "exit_rcu ps \<sigma> t ps' \<sigma>' \<equiv>  ps = ps' \<and> (\<exists>x.  (A ps x = Some (rcu_0, pointer))
-                                      \<and> (\<sigma> [ (rcu_0+t) := 0 ]\<^sub>t \<sigma>'))" 
-
-definition setup_r :: "mstate \<Rightarrow> T \<Rightarrow>  mstate \<Rightarrow> bool" ("_ r[N]:={0} _ _" [200])    \<comment>\<open>r[N] = {0}\<close>
-  where
-  "setup_r  ms t ms' \<equiv> ms' = ms \<lparr> r := (r ms) (t := \<lambda> i . 0),
-                                 pc := (pc ms) (t := S2)\<rparr>"
-
-
-
-
-
-
-
-
-(*\<forall>i. (i\<in> free_addrs) \<longleftrightarrow> rd_cap ms i = {} *)
-(*cannot take set wr_cap l ms :=t if wr_cap l ms=t*)
-(*must have rd_cap on l (t\<in>rd_cap l ms) to perform wr_cap l ms := t*)
-(*capabilities stuff
-definition relinquish_rd_cap :: "T \<Rightarrow> mstate \<Rightarrow> mstate" ("give\<^sub>u\<^sub>p _" [200])
-  where 
-  "relinquish_rd_cap t ms \<equiv> ms \<lparr> rd_cap := \<lambda> x. if  t\<in>rd_cap ms x  then rd_cap ms x - {t} else rd_cap ms x \<rparr>"
-
-definition take_rd_cap :: "L \<Rightarrow> T \<Rightarrow> mstate \<Rightarrow> mstate" ("take\<^sub>_ _" [200,200])
-  where 
-  "take_rd_cap l t ms \<equiv> ms \<lparr> rd_cap := (rd_cap ms) (l := ((rd_cap ms l) \<union> {t})) \<rparr>"
-*)(*decide where to put this^^^^^^^^^^^^^^^^^^^^^^^^^^^^^^^*)
-
-
-
-definition insert_address :: " mstate \<Rightarrow> T \<Rightarrow> nat \<Rightarrow> mstate \<Rightarrow> bool" ("_ insert[detached[_],_] _" [200,200,200,200])    \<comment>\<open>insert(_, s)\<close>
-  where
-  "insert_address ms t loc ms' \<equiv> ms' = ms\<lparr> det := (det ms) (t:= (((det ms) t) @ [loc])),
-                                            pc := (pc ms) (t := R2), 
-                                             s_dec := (s_dec ms) (t := False),
-                                             s := (s ms) (t := None)\<rparr>"
-
-
-definition nondet :: "mstate \<Rightarrow> T \<Rightarrow> bool \<Rightarrow> mstate \<Rightarrow> bool" ("_ nondet[_,_] _" [200,200,200,200])    \<comment>\<open>nondet()\<close>
-  where
-  "nondet ms t b ms' \<equiv> ms' = ms \<lparr> nondet_val := (nondet_val ms) (t:= b),
-                                          pc := (pc ms) (t := R3)\<rparr>"
-
-
-definition rcu_temp_copy :: "mstate \<Rightarrow> surrey_state \<Rightarrow> nat \<Rightarrow> T \<Rightarrow> mstate \<Rightarrow> surrey_state \<Rightarrow> bool" ( "_ _ load(_)\<^sub>_ _ _" [200,200,200,200,200,200])
-  where
-  "rcu_temp_copy ms \<sigma> ctr_val t ms' \<sigma>'\<equiv> \<exists> v. ((\<sigma> [ v \<leftarrow> (rcu_0 + ctr_val)]\<^sub>t \<sigma>')     \<comment>\<open>read rcu[i]\<close>
-                                        \<and> (ms' = ms\<lparr>reg := (reg ms) (t := v),
-                                                    pc := (pc ms) (t := S7)\<rparr>)) "
-
-definition cas_step_rcu :: "mstate \<Rightarrow> surrey_state \<Rightarrow>T \<Rightarrow> L \<Rightarrow> V \<Rightarrow> V \<Rightarrow> mstate \<Rightarrow>  surrey_state \<Rightarrow> bool" 
- where
-    "cas_step_rcu ms \<sigma> t l cv nv ms' \<sigma>'\<equiv>           \<comment>\<open>CAS(&C,s,n)\<close>
-       \<exists> w ts'. w \<in> visible_writes \<sigma> t l \<and>
-               w \<notin> covered \<sigma> \<and>
-               valid_fresh_ts \<sigma> w ts' \<and>
-       \<sigma>' = fst(CAS t w cv nv \<sigma> ts')    
-       \<and> 
-(snd(CAS t w cv nv \<sigma> ts') = True \<longrightarrow>(ms' = ms\<lparr>CAS_succ := (CAS_succ ms) (t := snd(CAS t w cv nv \<sigma> ts')),
-                                                 n_dec := (n_dec ms) (t := False),
-                                                  own\<^sub>W := (own\<^sub>W ms) (cv:=Some t),        \<comment>\<open>acquire wr_cap on location\<close>
-                                                  own\<^sub>W := (own\<^sub>W ms) (nv:=None),          \<comment>\<open>let go of wr_cap on location\<close>
-                                                   pc  := (pc ms) (t := cas_res)\<rparr>))
-       \<and> 
-(snd(CAS t w cv nv \<sigma> ts') = False \<longrightarrow>(ms' = ms\<lparr>CAS_succ := (CAS_succ ms) (t := snd(CAS t w cv nv \<sigma> ts')),
-                                                   pc := (pc ms) (t := cas_res)\<rparr>))"           
-
-
-
-
-
-
-definition inc_ctr1 :: "T \<Rightarrow> mstate \<Rightarrow> mstate" ( "CTRsync\<^sub>1[_]++" [200])
-  where
-  "inc_ctr1 t ms \<equiv>  ms \<lparr> CTRsync\<^sub>1 := (CTRsync\<^sub>1 ms) (t:=(CTRsync\<^sub>1 ms t)+1) \<rparr> "
-
-definition inc_ctr2 :: "T \<Rightarrow> mstate \<Rightarrow> mstate" ( "CTRsync\<^sub>2[_]++" [200])
-  where
-  "inc_ctr2 t ms \<equiv>  ms \<lparr> CTRsync\<^sub>2 := (CTRsync\<^sub>2 ms) (t:=(CTRsync\<^sub>2 ms t)+1) \<rparr> "
-
-definition update_ctr1 :: "T \<Rightarrow> nat \<Rightarrow> mstate \<Rightarrow> mstate" ( "CTRsync\<^sub>1[_]:=_" [200,200])
-  where
-  "update_ctr1 t ctr_val ms \<equiv> ms \<lparr> CTRsync\<^sub>1 := (CTRsync\<^sub>1 ms) (t:=ctr_val) \<rparr> "
-
-definition update_ctr2 :: "T \<Rightarrow> nat \<Rightarrow> mstate \<Rightarrow> mstate" ( "CTRsync\<^sub>2[_]:=_" [200,200])
-  where
-  "update_ctr2 t ctr_val ms \<equiv> ms \<lparr> CTRsync\<^sub>2 := (CTRsync\<^sub>2 ms) (t:=ctr_val) \<rparr> "
-
-definition update_pc :: "T \<Rightarrow> PC \<Rightarrow> mstate \<Rightarrow>  mstate" ( "pc[_]:=_" [200,200])
-  where
-  "update_pc t pc_val ms \<equiv>  ms \<lparr> pc := (pc ms) (t:=pc_val) \<rparr> "
-
-definition repetition :: "T \<Rightarrow> bool \<Rightarrow> mstate \<Rightarrow>  mstate" ( "repeat[_]:=_" [200,200])
-  where
-  "repetition t b ms \<equiv>  ms \<lparr> repeat := (repeat ms) (t:=b) \<rparr> "
-
-definition nallocdef :: "T \<Rightarrow> bool \<Rightarrow> mstate \<Rightarrow> mstate" ( "n[_]:=_" [200,200])
-  where
-  "nallocdef t b ms \<equiv>  ms \<lparr> n_dec := (n_dec ms) (t:=b) \<rparr> "
-
-definition sallocdef :: "T \<Rightarrow> bool \<Rightarrow> mstate \<Rightarrow> mstate" ( "s[_]:=_" [200,200])
-  where
-  "sallocdef t b ms \<equiv>  ms \<lparr> s_dec := (s_dec ms) (t:=b) \<rparr> "
-
-definition SC_fence :: "surrey_state \<Rightarrow> T \<Rightarrow> surrey_state \<Rightarrow> bool " ("_ Fence _ _" [200,200,200])
-  where
-  "SC_fence \<sigma> t \<sigma>' \<equiv> 
-       \<exists> w ts'. w \<in> visible_writes \<sigma> t casloc \<and>
-               w \<notin> covered \<sigma> \<and>
-               valid_fresh_ts \<sigma> w ts' \<and>
-       \<sigma>' = fst(CAS t w (value \<sigma> w) (value \<sigma> w) \<sigma> ts')"
-
-
-
-
-
-lemmas abbr = v_allocation_def int_star_n_def int_star_s_def
-                new_int_def get_s_def writeto_star_n_def
-                pop_address_def
-                load_rcu_to_r_def 
-                enter_rcu_def exit_rcu_def
-                setup_r_def
-                insert_address_def nondet_def
-                rcu_temp_copy_def cas_step_rcu_def
-                inc_ctr1_def inc_ctr2_def update_ctr1_def update_ctr2_def update_pc_def
-                repetition_def SC_fence_def
-                sallocdef_def nallocdef_def
-                giveup_readandwrite_ownership_def
-
-
-
-(*==========================   Thread behaviour   =================================*)
-
-section \<open>Program step\<close>
-definition step :: "mstate \<Rightarrow> posem \<Rightarrow> surrey_state \<Rightarrow>  PC \<Rightarrow> T \<Rightarrow>  mstate \<Rightarrow> posem \<Rightarrow> surrey_state \<Rightarrow> bool " where
-"step ms ps \<sigma> pcr t ms' ps' \<sigma>' \<equiv> 
-case pcr of 
-   R1 \<Rightarrow> (ms insert[detached[t],the (s ms t)] ms') \<and> ps = ps' \<and> \<sigma> =\<sigma>' 
-|  R2 \<Rightarrow> (\<exists>b. (b\<in>{True,False} \<and> (ms nondet[t,b] ms'))) \<and> ps = ps' \<and> \<sigma> =\<sigma>' 
-|  R3 \<Rightarrow> if (nondet_val ms t) = True 
-            then ms' = (pc[t]:=S1) ms  \<and> ps = ps' \<and> \<sigma> =\<sigma>'  
-               \<comment>\<open> sync() \<close>
-            else ms' = (pc[t]:=I13) ms  \<and> ps = ps' \<and> \<sigma> =\<sigma>'  
-               \<comment>\<open> return to inc() \<close>
-|  R4 \<Rightarrow> if (det ms t \<noteq> [])
-            then ms' = (pc[t]:=R5)  ms  \<and> ps = ps' \<and> \<sigma> =\<sigma>'  
-            else ms' = (pc[t]:=I13) ms  \<and> ps = ps' \<and> \<sigma> =\<sigma>'     \<comment>\<open> return to inc() \<close>
-\<comment>\<open> \<close>
-|  R5 \<Rightarrow> (ms ps free[pop[detached[t]]] ms' ps')  \<and> \<sigma> =\<sigma>'                  \<comment>\<open> ownW ps hd(det ps t) := None \<close>
-\<comment>\<open> \<close>
-|  S1 \<Rightarrow> (ms r[N]:={0} t ms') \<and> ps = ps'  \<and> \<sigma> = \<sigma>'
-|  S2 \<Rightarrow> if (CTRsync\<^sub>1 ms t < T_max)
-            then ms' = (CTRsync\<^sub>1[t]++ \<circ> pc[t]:=S3) ms \<and> ps = ps' \<and> \<sigma> =\<sigma>'
-            else ms' = (pc[t]:=S4) ms \<and> ps = ps' \<and> \<sigma> =\<sigma>'
-|  S3 \<Rightarrow> (ms ps \<sigma> r[i]:=rcu[i] t ms' ps' \<sigma>')
-|  S4 \<Rightarrow> if (CTRsync\<^sub>2 ms t < T_max)
-            then ms' = (pc[t]:=S5) ms \<and> ps = ps' \<and> \<sigma> =\<sigma>'
-            else ms' = (pc[t]:=R4) ms \<and> ps = ps' \<and> \<sigma> =\<sigma>'        \<comment>\<open> return to Reclaim (R4)\<close>
-|  S5 \<Rightarrow> if r ms t (CTRsync\<^sub>2 ms t) = 0
-            then ms' = (CTRsync\<^sub>2[t]++ \<circ> pc[t]:=S4) ms \<and> ps = ps' \<and> \<sigma> =\<sigma>'
-            else ms' = (pc[t]:=S6) ms \<and> ps = ps' \<and> \<sigma> =\<sigma>'
-|  S6 \<Rightarrow> ms \<sigma> load(CTRsync\<^sub>2 ms t)\<^sub>t ms' \<sigma>' \<and> ps = ps'  \<comment>\<open> load \<langle>rcu[i]\<rangle> into reg, increment pc\<close>
-|  S7 \<Rightarrow> if reg ms t = 1                             \<comment>\<open> test while \<langle>rcu[i]\<rangle>\<close>
-            then ms' = (pc[t]:=S6) ms \<and> ps = ps' \<and> \<sigma> =\<sigma>'
-            else ms' = (CTRsync\<^sub>2[t]++ \<circ> pc[t]:=S4) ms \<and> ps = ps' \<and> \<sigma> =\<sigma>'
-
-
-|  I1  \<Rightarrow> (ms int[v\<^sub>t] ms')  \<and> ps = ps' \<and> \<sigma> = \<sigma>'
-|  I2  \<Rightarrow> (ms int[*n\<^sub>t] ms') \<and> ps = ps' \<and> \<sigma> = \<sigma>'
-|  I3  \<Rightarrow> (ms int[*s\<^sub>t] ms') \<and> ps = ps' \<and> \<sigma> = \<sigma>'
-|  I4  \<Rightarrow> (ms ps n:=newint t ms' ps')  \<and> \<sigma> = \<sigma>'                                           \<comment>\<open> takes raw cap on n\<close>
-|  I5  \<Rightarrow> (ps \<sigma> rcuenter[] t ps' \<sigma>') \<and> (ms' = (pc[t]:=I6) ms)
-|  I6  \<Rightarrow> (ps \<sigma> rcuexit[] t ps' \<sigma>')  \<and> (ms' = (pc[t]:=I7 \<circ> givesupRown[t,the (s ms t)]) ms)   \<comment>\<open> lets go of raw cap on s\<close>
-|  I7  \<Rightarrow> (ps \<sigma> rcuenter[] t ps' \<sigma>') \<and> (ms' = (pc[t]:=I8) ms)
-\<comment>\<open>|  fence \<Rightarrow>  (\<sigma> Fence t \<sigma>') \<and> ps = ps' \<and> (ms' = (pc[t]:=I8) ms)   SC fence \<close> 
-|  I8  \<Rightarrow> (ms \<sigma> s:=\<^sup>FC t ms' \<sigma>')       \<and> ps = ps'          \<comment>\<open> Fetch and Add 0 \<close>            \<comment>\<open> takes r cap on s (C weak read)\<close>
-|  I9  \<Rightarrow> (ms \<sigma> v:=*s t ms' \<sigma>')      \<and> ps = ps'     
-|  I10 \<Rightarrow> (ms \<sigma> *n:=newv t ms' \<sigma>')   \<and> ps = ps'                  \<comment>\<open> (ownW ps n) = t \<close>
-|  I11 \<Rightarrow> cas_step_rcu ms \<sigma> t C (the (s ms t)) (the (n ms t)) ms' \<sigma>' \<and> ps = ps'           \<comment>\<open> swaps wr cap from n to s\<close>
-|  cas_res \<Rightarrow> if CAS_succ ms t 
-            then (ms' = (pc[t]:=I12) ms) \<and> ps = ps' \<and> \<sigma> = \<sigma>'
-            else (ms' = (pc[t]:=I6 \<circ> repeat[t]:=True) ms) \<and> ps = ps' \<and> \<sigma> = \<sigma>'
-|  I12 \<Rightarrow> (ps \<sigma> rcuexit[] t ps' \<sigma>') \<and> (ms' = ((pc[t]:=R1 \<circ> n[t]:=False \<circ> givesupRown[t,the (n ms t)])) ms)  \<comment>\<open> lets go of raw cap on n\<close>
-        \<comment>\<open>reclaim(s)\<close>                                            \<comment>\<open> (ownW ps s) = t \<close>            \<comment>\<open> lets go of raw cap on s\<close>
-|  I13 \<Rightarrow> (ms' = (pc[t]:=I14) ms) \<and> \<sigma> = \<sigma>' \<and> ps = ps'   
-|  I14 \<Rightarrow> ms' = (repeat[t]:=False) ms \<and> \<sigma> = \<sigma>' \<and> ps = ps'  \<comment>\<open> return(v) \<close> 
-| finished \<Rightarrow> ms = ms' \<and> ps=ps' \<and> \<sigma>=\<sigma>'
-" 
-
-lemma "n ms' t \<noteq> i \<Longrightarrow> (SOME loc. (the(n ms' t) = loc)) \<equiv> the(n ms' t)"
-  by simp
-  
-
-  
-lemma " \<exists> x. (x=2 \<and> x = p) \<Longrightarrow>  (SOME x.  x)  \<equiv> p=2 "
-  by (simp add: some_equality)
-
-
-
-
-
-
-
-definition "Rcap ms t addrs \<equiv> \<forall>i. (i\<in>addrs) \<longleftrightarrow> (t\<in>own\<^sub>R ms i)"
-definition "Wcap ms t addrs \<equiv> \<forall>i. (i\<in>addrs) \<longleftrightarrow> (the(own\<^sub>W ms i)=t)"
-
-definition "inlist a lst \<equiv> \<exists>j.(j<length(lst) \<and> lst!j = a)"
-definition "detaddrs ms t \<equiv> {i. inlist i (det ms t)}"
-definition "tail_detaddrs ms t \<equiv> {i. inlist i (det ms t)}"
-definition "n_pointer ms t\<equiv> the(n ms t)"
-definition "s_pointer ms t\<equiv> the(s ms t)"
-definition "s_and_n ms t \<equiv> {n_pointer ms t,s_pointer ms t}"
-definition "just_n ms t \<equiv> {n_pointer ms t}"
-definition "just_s ms t \<equiv> {s_pointer ms t}"
-
-(*\<forall>t loc. t\<le>T_max \<and> loc\<noteq>s_t \<and> loc\<noteq>n_t \<and> loc \<notin> detaddrs ms t \<and> loc\<noteq>C \<and> loc\<noteq>rcu[t]\<longrightarrow> loc\<in>free *)
-(*\<forall>loc. loc\<in>free \<longrightarrow> own\<^sub>R ms loc = {}*)
-lemmas names [simp] = n_pointer_def s_pointer_def s_and_n_def just_n_def just_s_def
-                      inlist_def detaddrs_def tail_detaddrs_def
-lemmas names_2      = Rcap_def Wcap_def
-
-
-(*------------structure lemmas---------------*)
-
-definition "addr_allocated ms ps \<equiv> \<forall>addr t . addr \<in> detaddrs ms t \<longrightarrow> 
-                                 (\<exists>prov. (A ps prov = Some (addr, pointer)))"
-
-definition "nptr_true_imp ms ps \<equiv> \<forall>t . (n_dec ms t = True \<and> n ms t\<noteq>None) \<longrightarrow>
-                          (\<exists>prov. (A ps prov = Some (the (n ms t), pointer)))"
-
-definition "sptr_true_imp ms ps \<equiv> \<forall>t . (s_dec ms t = True \<and> s ms t\<noteq>None) \<longrightarrow>
-                          (\<exists>prov. (A ps prov = Some (the (s ms t), pointer)))"
-
-(*-----------observation lemmas --------------*)
-
-
-
-
-
-
-(*------- careful observation of preCond per thread ----------*)
-definition "pre_I1 ms t \<equiv>
-                         Rcap ms t (detaddrs ms t) \<and> Wcap ms t (detaddrs ms t)
-                       \<and> n ms t = None 
-                       \<and> n_dec ms t = False
-"
-
-(* s ms t = None
-                        
-                        \<and> v ms t = None
-                        \<and> s ms t = False 
-                        \<and> n ms t = False 
-                        \<and> CTRsync\<^sub>1 ms t = 0 \<and> CTRsync\<^sub>2 ms t = 0 
-                        \<and> res ms t = 0 \<and> reg ms t = 0
-                        \<and> nondet_val ms t = False \<and> CAS_succ ms t = False \<and> repeat ms t = False
-                        \<and> *)
-definition "pre_I2 ms t \<equiv>
-                          Rcap ms t (detaddrs ms t) \<and> Wcap ms t (detaddrs ms t)
-                        \<and> n ms t = None 
-                        \<and> n_dec ms t = True
-"
-(*s ms t = None 
-                        \<and> n ms t = None 
-                        \<and> v ms t = None
-                        \<and> s ms t = False 
-                        \<and> n_dec ms t = False 
-                        \<and> CTRsync\<^sub>1 ms t = 0 \<and> CTRsync\<^sub>2 ms t = 0 
-                        \<and> res ms t = 0 \<and> reg ms t = 0
-                        \<and> nondet_val ms t = False \<and> CAS_succ ms t = False \<and> repeat ms t = False
-                        \<and> *)
-definition "pre_I3 ms t \<equiv>
-                         Rcap ms t (detaddrs ms t) \<and> Wcap ms t (detaddrs ms t)
-                       \<and> n ms t = None 
-                       \<and> n_dec ms t = True
-"
-(*s ms t = None 
-                        \<and> n ms t = None 
-                        \<and> v ms t = None
-                        \<and> s ms t = False
-                        \<and> n ms t = True 
-                        \<and> CTRsync\<^sub>1 ms t = 0 \<and> CTRsync\<^sub>2 ms t = 0 
-                        \<and> res ms t = 0 \<and> reg ms t = 0
-                        \<and> nondet_val ms t = False \<and> CAS_succ ms t = False \<and> repeat ms t = False
-                        \<and>*)
-definition "pre_I4 ms t \<equiv>
-                          Rcap ms t (detaddrs ms t) \<and> Wcap ms t (detaddrs ms t)
-                       \<and> n ms t = None 
-                       \<and> n_dec ms t = True
-"
-(*s ms t = None
-                        \<and> n ms t = None
-                        \<and> v ms t = None
-                        \<and> s ms t = True
-                        \<and> n ms t = True
-                        \<and> CTRsync\<^sub>1 ms t = 0 \<and> CTRsync\<^sub>2 ms t = 0 
-                        \<and> res ms t = 0 \<and> reg ms t = 0
-                        \<and> nondet_val ms t = False \<and> CAS_succ ms t = False \<and> repeat ms t = False
-                        \<and> *)
-definition "pre_I5 ms t \<equiv>
-                           Rcap ms t (detaddrs ms t \<union> just_n ms t) \<and> Wcap ms t (detaddrs ms t \<union> just_n ms t)
-                       \<and> n ms t \<noteq> None 
-                       \<and> n_dec ms t = True
-"
-(*s ms t = None
-                        \<and> (\<exists>i. n ms t = Some i)
-                        \<and> v ms t = None
-                        \<and> s ms t = True
-                        \<and> n ms t = True
-                        \<and> CTRsync\<^sub>1 ms t = 0 \<and> CTRsync\<^sub>2 ms t = 0 
-                        \<and> res ms t = 0 \<and> reg ms t = 0
-                        \<and> nondet_val ms t = False \<and> CAS_succ ms t = False \<and> repeat ms t = False
-                        \<and>*)
-definition "pre_I6 ms t \<equiv>
-                         Wcap ms t (detaddrs ms t \<union> just_n ms t) 
-                \<and>  repeat ms t  \<longrightarrow>(s ms t \<noteq> None \<and> Rcap ms t (detaddrs ms t \<union> s_and_n ms t))
-                \<and> \<not>repeat ms t  \<longrightarrow>(s ms t = None \<and> Rcap ms t (detaddrs ms t \<union> just_n ms t))
-                       \<and> n ms t \<noteq> None 
-                       \<and> n_dec ms t = True
-"
-(*(repeat ms t  \<longrightarrow> (\<exists>j k. s ms t = Some j \<and> v ms t = Some k))
-                        \<and> (\<not>repeat ms t \<longrightarrow> s ms t = None \<and> v ms t = None
-                                          \<and> Rcap ms t (detaddrs ms t \<union> just_n ms t))
-                        \<and> (\<exists>i. n ms t = Some i)
-                        \<and> s ms t = True
-                        \<and> n ms t = True
-                        \<and> CTRsync\<^sub>1 ms t = 0 \<and> CTRsync\<^sub>2 ms t = 0 
-                        \<and> res ms t = 0 \<and> reg ms t = 0
-                        \<and> nondet_val ms t = False \<and> CAS_succ ms t = False 
-                        \<and>*)
-definition "pre_I7 ms t \<equiv>
-                          Rcap ms t (detaddrs ms t \<union> just_n ms t) \<and> Wcap ms t (detaddrs ms t \<union> just_n ms t)
-                       \<and> n ms t \<noteq> None 
-                       \<and> n_dec ms t = True
-"
-(*(\<not>repeat ms t \<longrightarrow> s ms t = None \<and> v ms t = None)
-                        \<and> (repeat ms t \<longrightarrow> (\<exists>j k. s ms t = Some j \<and> v ms t = Some k))
-                        \<and> (\<exists>i. n ms t = Some i)
-                        \<and> s ms t = True
-                        \<and> n ms t = True
-                        \<and> CTRsync\<^sub>1 ms t = 0 \<and> CTRsync\<^sub>2 ms t = 0 
-                        \<and> res ms t = 0 \<and> reg ms t = 0
-                        \<and> nondet_val ms t = False \<and> CAS_succ ms t = False 
-                        \<and> *)
-definition "pre_I8 ms t \<equiv> 
-                           Rcap ms t (detaddrs ms t \<union> just_n ms t) \<and> Wcap ms t (detaddrs ms t \<union> just_n ms t)
-                       \<and> n ms t \<noteq> None 
-                       \<and> n_dec ms t = True
-"
-(*(\<not>repeat ms t \<longrightarrow> s ms t = None \<and> v ms t = None)
-                        \<and> (repeat ms t \<longrightarrow> (\<exists>j k. s ms t = Some j \<and> v ms t = Some k))
-                        \<and> (\<exists>i. n ms t = Some i)
-                        \<and> s ms t = True
-                        \<and> n ms t = True
-                        \<and> CTRsync\<^sub>1 ms t = 0 \<and> CTRsync\<^sub>2 ms t = 0 
-                        \<and> res ms t = 0 \<and> reg ms t = 0
-                        \<and> nondet_val ms t = False \<and> CAS_succ ms t = False
-                        \<and>*)
-definition "pre_I9 ms t \<equiv> 
-                           Rcap ms t (detaddrs ms t \<union> s_and_n ms t) \<and> Wcap ms t (detaddrs ms t \<union> just_n ms t)
-                       \<and> n ms t \<noteq> None 
-                       \<and> n_dec ms t = True
-"
-(*(\<not>repeat ms t \<longrightarrow>  v ms t = None)
-                        \<and> (repeat ms t \<longrightarrow> (\<exists>k. v ms t = Some k))
-                        \<and> (\<exists>j. s ms t = Some j)
-                        \<and> (\<exists>i. n ms t = Some i)
-                        \<and> s ms t = True
-                        \<and> n ms t = True
-                        \<and> CTRsync\<^sub>1 ms t = 0 \<and> CTRsync\<^sub>2 ms t = 0 
-                        \<and> res ms t = 0 \<and> reg ms t = 0
-                        \<and> nondet_val ms t = False \<and> CAS_succ ms t = False 
-                        \<and>*)
-definition "pre_I10 ms t \<equiv>
-                           Rcap ms t (detaddrs ms t \<union> s_and_n ms t) \<and> Wcap ms t (detaddrs ms t \<union> just_n ms t)
-                       \<and> n ms t \<noteq> None 
-                       \<and> n_dec ms t = True
-"
-(*(\<exists>j. s ms t = Some j)
-                        \<and> (\<exists>i. n ms t = Some i)
-                        \<and> (\<exists>k. v ms t = Some k)
-                        \<and> s ms t = True
-                        \<and> n ms t = True
-                        \<and> CTRsync\<^sub>1 ms t = 0 \<and> CTRsync\<^sub>2 ms t = 0 
-                        \<and> res ms t = 0 \<and> reg ms t = 0
-                        \<and> nondet_val ms t = False \<and> CAS_succ ms t = False
-                        \<and>*)
-definition "pre_I11 ms t \<equiv>
-                          Rcap ms t (detaddrs ms t \<union> s_and_n ms t) \<and> Wcap ms t (detaddrs ms t \<union> just_n ms t)
-                       \<and> n ms t \<noteq> None 
-                       \<and> n_dec ms t = True
-"
-(*(\<exists>j. s ms t = Some j)
-                        \<and> (\<exists>i. n ms t = Some i)
-                        \<and> (\<exists>k. v ms t = Some k)
-                        \<and> s ms t = True
-                        \<and> n ms t = True
-                        \<and> CTRsync\<^sub>1 ms t = 0 \<and> CTRsync\<^sub>2 ms t = 0 
-                        \<and> res ms t = 0 \<and> reg ms t = 0
-                        \<and> nondet_val ms t = False \<and> CAS_succ ms t = False
-                        \<and> *)
-definition "pre_cas_res ms t \<equiv>
-                          (CAS_succ ms t \<longrightarrow> Rcap ms t (detaddrs ms t \<union> s_and_n ms t) \<and> Wcap ms t (detaddrs ms t \<union> just_s ms t)
-                       \<and> n_dec ms t)
-                        \<and> (\<not>CAS_succ ms t\<longrightarrow> Rcap ms t (detaddrs ms t \<union> s_and_n ms t) \<and> Wcap ms t (detaddrs ms t \<union> just_n ms t)
-                       \<and> \<not>n_dec ms t)
-                       \<and> n ms t \<noteq> None 
-"
-(*(\<exists>j. s ms t = Some j)
-                        \<and> (\<exists>i. n ms t = Some i)
-                        \<and> (\<exists>k. v ms t = Some k)
-                        \<and> s ms t = True
-                        \<and> n ms t = True
-                        \<and> CTRsync\<^sub>1 ms t = 0 \<and> CTRsync\<^sub>2 ms t = 0 
-                        \<and> res ms t = 0 \<and> reg ms t = 0
-                        \<and> nondet_val ms t = False 
-                        \<and> *)
-definition "pre_I12 ms t \<equiv>
-                           Rcap ms t (detaddrs ms t \<union> s_and_n ms t) \<and> Wcap ms t (detaddrs ms t \<union> just_s ms t)
-                       \<and> \<not>n_dec ms t
-                       \<and> n ms t \<noteq> None 
-"
-(*(\<exists>j. s ms t = Some j)
-                        \<and> (\<exists>i. n ms t = Some i)
-                        \<and> (\<exists>k. v ms t = Some k)
-                        \<and> s ms t = True
-                        \<and> n ms t = True
-                        \<and> CTRsync\<^sub>1 ms t = 0 \<and> CTRsync\<^sub>2 ms t = 0 
-                        \<and> res ms t = 0 \<and> reg ms t = 0
-                        \<and> nondet_val ms t = False \<and> CAS_succ ms t = True
-                        \<and>*)
-\<comment>\<open> start to reclaim() \<close>
-definition "pre_I13 ms t \<equiv>
-                          Rcap ms t (detaddrs ms t) \<and> Wcap ms t (detaddrs ms t)
-                       \<and> \<not>n_dec ms t
-                       \<and> n ms t \<noteq> None 
-"
-(*(\<exists>j. s ms t = Some j)
-                        \<and> (\<exists>i. n ms t = Some i)
-                        \<and> (\<exists>k. v ms t = Some k)
-                        \<and> s ms t = False
-                        \<and> n ms t = False
-                        \<and> CTRsync\<^sub>1 ms t = T_max \<and> CTRsync\<^sub>2 ms t = T_max
-                        \<and> res ms t = 0 
-                        \<and> nondet_val ms t = False \<and> CAS_succ ms t = True
-                        \<and> *)
-definition "pre_I14 ms t \<equiv>
-                           Rcap ms t (detaddrs ms t) \<and> Wcap ms t (detaddrs ms t)
-                       \<and> \<not>n_dec ms t
-                       \<and> n ms t \<noteq> None 
-"
-(*(\<exists>j. s ms t = Some j)
-                        \<and> (\<exists>i. n ms t = Some i)
-                        \<and> (\<exists>k. v ms t = Some k)
-                        \<and> s ms t = False
-                        \<and> n ms t = False
-                        \<and> CTRsync\<^sub>1 ms t = T_max \<and> CTRsync\<^sub>2 ms t = T_max
-                        \<and> res ms t = 0 
-                        \<and> nondet_val ms t = False \<and> CAS_succ ms t = True
-                        \<and>*)
-
-
-definition "pre_R1 ms t \<equiv>  
-                           Rcap ms t (detaddrs ms t \<union> just_s ms t) \<and> Wcap ms t (detaddrs ms t \<union> just_s ms t)
-                       \<and> \<not>n_dec ms t
-                       \<and> n ms t \<noteq> None 
-"
-(*(\<exists>j. s ms t = Some j)
-                        \<and> (\<exists>i. n ms t = Some i)
-                        \<and> (\<exists>k. v ms t = Some k)
-                        \<and> s ms t = True
-                        \<and> n ms t = False
-                        \<and> CTRsync\<^sub>1 ms t = 0 \<and> CTRsync\<^sub>2 ms t = 0 
-                        \<and> res ms t = 0 \<and> reg ms t = 0
-                        \<and> nondet_val ms t = False \<and> CAS_succ ms t = True
-                        \<and>*)
-definition "pre_R2 ms t \<equiv>
-                           Rcap ms t (detaddrs ms t) \<and> Wcap ms t (detaddrs ms t)
-                       \<and> \<not>n_dec ms t
-                       \<and> n ms t \<noteq> None 
-"
-(*(\<exists>j. s ms t = Some j)
-                        \<and> (\<exists>i. n ms t = Some i)
-                        \<and> (\<exists>k. v ms t = Some k)
-                        \<and> s ms t = False
-                        \<and> n ms t = False
-                        \<and> just_s ms t \<in> {detaddrs ms t}         \<comment> \<open>s union detatched addresses\<close>
-                        \<and> CTRsync\<^sub>1 ms t = 0 \<and> CTRsync\<^sub>2 ms t = 0 
-                        \<and> res ms t = 0 \<and> reg ms t = 0
-                        \<and> nondet_val ms t = False \<and> CAS_succ ms t = True
-                        \<and>*)
-definition "pre_R3 ms t \<equiv>
-                           Rcap ms t (detaddrs ms t) \<and> Wcap ms t (detaddrs ms t)
-                       \<and> \<not>n_dec ms t
-                       \<and> n ms t \<noteq> None 
-"
-(*(\<exists>j. s ms t = Some j)
-                        \<and> (\<exists>i. n ms t = Some i)
-                        \<and> (\<exists>k. v ms t = Some k)
-                        \<and> s ms t = False
-                        \<and> n ms t = False
-                        \<and> just_s ms t \<in> {detaddrs ms t}         \<comment> \<open>s union detatched addresses\<close>
-                        \<and> CTRsync\<^sub>1 ms t = 0 \<and> CTRsync\<^sub>2 ms t = 0 
-                        \<and> res ms t = 0 \<and> reg ms t = 0
-                        \<and> CAS_succ ms t = True                  \<comment> \<open>random nondet_val picked\<close>
-                        \<and>*)
-\<comment>\<open> start to sync() \<close>
-\<comment>\<open> or return to inc() \<close>
-definition "pre_R4 ms t \<equiv>  
-                           Rcap ms t (detaddrs ms t) \<and> Wcap ms t (detaddrs ms t)
-                       \<and> \<not>n_dec ms t
-                       \<and> n ms t \<noteq> None 
-"
-(*(\<exists>j. s ms t = Some j)
-                        \<and> (\<exists>i. n ms t = Some i)
-                        \<and> (\<exists>k. v ms t = Some k)
-                        \<and> s ms t = False
-                        \<and> n ms t = False
-                        \<and> CTRsync\<^sub>1 ms t = T_max \<and> CTRsync\<^sub>2 ms t = T_max 
-                        \<and> res ms t = 0 \<and> reg ms t = 0
-                        \<and> nondet_val ms t = True \<and> CAS_succ ms t = True                  \<comment> \<open>random nondet_val picked\<close>
-                        \<and>*)
-\<comment>\<open> return to inc() \<close>
-definition "pre_R5 ms t \<equiv>
-                           Rcap ms t (detaddrs ms t) \<and> Wcap ms t (detaddrs ms t)
-                       \<and> \<not>n_dec ms t
-                       \<and> n ms t \<noteq> None 
-"
-(*(\<exists>j. s ms t = Some j)
-                        \<and> (\<exists>i. n ms t = Some i)
-                        \<and> (\<exists>k. v ms t = Some k)
-                        \<and> s ms t = False
-                        \<and> n ms t = False
-                        \<and> det ms t \<noteq> []
-                        \<and> CTRsync\<^sub>1 ms t = T_max \<and> CTRsync\<^sub>2 ms t = T_max 
-                        \<and> res ms t = 0 \<and> reg ms t = 0
-                        \<and> nondet_val ms t = True \<and> CAS_succ ms t = True                  \<comment> \<open>random nondet_val picked\<close>
-                        \<and>*)
-
-
-definition "pre_S1 ms t \<equiv>  
-                           Rcap ms t (detaddrs ms t) \<and> Wcap ms t (detaddrs ms t)
-                       \<and> \<not>n_dec ms t
-                       \<and> n ms t \<noteq> None 
-"
-(*(\<exists>j. s ms t = Some j)
-                        \<and> (\<exists>i. n ms t = Some i)
-                        \<and> (\<exists>k. v ms t = Some k)
-                        \<and> s ms t = False
-                        \<and> n ms t = False
-                        \<and> just_s ms t \<in> {detaddrs ms t}         \<comment> \<open>s union detatched addresses\<close>
-                        \<and> CTRsync\<^sub>1 ms t = 0 \<and> CTRsync\<^sub>2 ms t = 0 
-                        \<and> res ms t = 0 \<and> reg ms t = 0
-                        \<and> nondet_val ms t = True \<and> CAS_succ ms t = True 
-                        \<and>*)
-definition "pre_S2 ms t \<equiv>
-                           Rcap ms t (detaddrs ms t) \<and> Wcap ms t (detaddrs ms t)
-                       \<and> \<not>n_dec ms t
-                       \<and> n ms t \<noteq> None 
-"
-(*(\<exists>j. s ms t = Some j)
-                        \<and> (\<exists>i. n ms t = Some i)
-                        \<and> (\<exists>k. v ms t = Some k)
-                        \<and> s ms t = False
-                        \<and> n ms t = False
-                        \<and> just_s ms t \<in> {detaddrs ms t}         \<comment> \<open>s union detatched addresses\<close>
-                        \<and> CTRsync\<^sub>1 ms t \<le> T_max \<and> CTRsync\<^sub>2 ms t = 0 
-                        \<and> res ms t = 0 \<and> reg ms t = 0
-                        \<and> nondet_val ms t = True \<and> CAS_succ ms t = True 
-                        \<and> (\<forall>i. (i>CTRsync\<^sub>1 ms t \<and> i\<le>T_max) \<longrightarrow> r ms t i = 0)        \<comment> \<open>local rcu register\<close>
-                        \<and>*)
-definition "pre_S3 ms t \<equiv>
-                           Rcap ms t (detaddrs ms t) \<and> Wcap ms t (detaddrs ms t)
-                       \<and> \<not>n_dec ms t
-                       \<and> n ms t \<noteq> None 
-"
-(*(\<exists>j. s ms t = Some j)
-                        \<and> (\<exists>i. n ms t = Some i)
-                        \<and> (\<exists>k. v ms t = Some k)
-                        \<and> s ms t = False
-                        \<and> n ms t = False
-                        \<and> just_s ms t \<in> {detaddrs ms t}         \<comment> \<open>s union detatched addresses\<close>
-                        \<and> CTRsync\<^sub>1 ms t \<le> T_max \<and> CTRsync\<^sub>2 ms t = 0 
-                        \<and> res ms t = 0 \<and> reg ms t = 0
-                        \<and> nondet_val ms t = True \<and> CAS_succ ms t = True 
-                        \<and> (\<forall>i. (i\<ge>CTRsync\<^sub>1 ms t \<and> i\<le>T_max) \<longrightarrow> r ms t i = 0)        \<comment> \<open>local rcu register\<close>
-                        \<and>*)
-definition "pre_S4 ms t \<equiv>
-                           Rcap ms t (detaddrs ms t) \<and> Wcap ms t (detaddrs ms t)
-                       \<and> \<not>n_dec ms t
-                       \<and> n ms t \<noteq> None 
-"
-(*(\<exists>j. s ms t = Some j)
-                        \<and> (\<exists>i. n ms t = Some i)
-                        \<and> (\<exists>k. v ms t = Some k)
-                        \<and> s ms t = False
-                        \<and> n ms t = False
-                        \<and> just_s ms t \<in> {detaddrs ms t}         \<comment> \<open>s union detatched addresses\<close>
-                        \<and> CTRsync\<^sub>1 ms t = T_max \<and> CTRsync\<^sub>2 ms t \<le> T_max 
-                        \<and> res ms t = 0 \<and> reg ms t = 0
-                        \<and> nondet_val ms t = True \<and> CAS_succ ms t = True 
-                        \<and> (\<forall>i. (i\<ge>CTRsync\<^sub>1 ms t \<and> i\<le>T_max) \<longrightarrow> r ms t i = 0)        \<comment> \<open>careful, here is smth to do with observations in wm\<close>
-                        \<and>*)
-definition "pre_S5 ms t \<equiv>
-                           Rcap ms t (detaddrs ms t) \<and> Wcap ms t (detaddrs ms t)
-                       \<and> \<not>n_dec ms t
-                       \<and> n ms t \<noteq> None 
-"
-(*(\<exists>j. s ms t = Some j)
-                        \<and> (\<exists>i. n ms t = Some i)
-                        \<and> (\<exists>k. v ms t = Some k)
-                        \<and> s ms t = False
-                        \<and> n ms t = False
-                        \<and> just_s ms t \<in> {detaddrs ms t}         \<comment> \<open>s union detatched addresses\<close>
-                        \<and> CTRsync\<^sub>1 ms t = T_max \<and> CTRsync\<^sub>2 ms t \<le> T_max 
-                        \<and> res ms t = 0 \<and> reg ms t = 0
-                        \<and> nondet_val ms t = True \<and> CAS_succ ms t = True 
-                        \<and> (\<forall>i. (i\<ge>CTRsync\<^sub>1 ms t \<and> i\<le>T_max) \<longrightarrow> r ms t i = 0)        \<comment> \<open>careful, here is smth to do with observations in wm\<close>
-                        \<and>*)
-definition "pre_S6 ms t \<equiv>
-                           Rcap ms t (detaddrs ms t) \<and> Wcap ms t (detaddrs ms t)
-                       \<and> \<not>n_dec ms t
-                       \<and> n ms t \<noteq> None 
-"
-(*(\<exists>j. s ms t = Some j)
-                        \<and> (\<exists>i. n ms t = Some i)
-                        \<and> (\<exists>k. v ms t = Some k)
-                        \<and> s ms t = False
-                        \<and> n ms t = False
-                        \<and> just_s ms t \<in> {detaddrs ms t}         \<comment> \<open>s union detatched addresses\<close>
-                        \<and> CTRsync\<^sub>1 ms t = T_max \<and> CTRsync\<^sub>2 ms t \<le> T_max 
-                        \<and> res ms t = 0 \<and> reg ms t = 0
-                        \<and> nondet_val ms t = True \<and> CAS_succ ms t = True 
-                        \<and> (\<forall>i. (i\<ge>CTRsync\<^sub>1 ms t \<and> i\<le>T_max) \<longrightarrow> r ms t i = 0)        \<comment> \<open>careful, here is smth to do with observations in wm\<close>
-                        \<and> r ms t (CTRsync\<^sub>2 ms t) = 1
-                        \<and>*)
-definition "pre_S7 ms t \<equiv>
-                          Rcap ms t (detaddrs ms t) \<and> Wcap ms t (detaddrs ms t)
-                       \<and> \<not>n_dec ms t
-                       \<and> n ms t \<noteq> None 
-"
-(*(\<exists>j. s ms t = Some j)
-                        \<and> (\<exists>i. n ms t = Some i)
-                        \<and> (\<exists>k. v ms t = Some k)
-                        \<and> s ms t = False
-                        \<and> n ms t = False
-                        \<and> just_s ms t \<in> {detaddrs ms t}         \<comment> \<open>s union detatched addresses\<close>
-                        \<and> CTRsync\<^sub>1 ms t = T_max \<and> CTRsync\<^sub>2 ms t \<le> T_max 
-                        \<and> res ms t = 0 
-                        \<and> (reg ms t = 0 \<or> reg ms t = 1) \<comment> \<open>this is basically TRUE/FALSE\<close>
-                        \<and> nondet_val ms t = True \<and> CAS_succ ms t = True 
-                        \<and> (\<forall>i. (i\<ge>CTRsync\<^sub>1 ms t \<and> i\<le>T_max) \<longrightarrow> r ms t i = 0)        \<comment> \<open>careful, here is smth to do with observations in wm\<close>
-                        \<and> r ms t (CTRsync\<^sub>2 ms t) = 1
-                        \<and> *)
-
-
-
-
-definition preCond :: "mstate \<Rightarrow> posem \<Rightarrow> surrey_state \<Rightarrow> PC \<Rightarrow> T \<Rightarrow> bool" where
-"preCond ms ps \<sigma> pcr t \<equiv> 
-case pcr of
-   I1 \<Rightarrow> pre_I1 ms t
-|  I2 \<Rightarrow> pre_I2 ms t
-|  I3 \<Rightarrow> pre_I3 ms t
-|  I4 \<Rightarrow> pre_I4 ms t
-|  I5 \<Rightarrow> pre_I5 ms t
-|  I6 \<Rightarrow> pre_I6 ms t
-|  I7 \<Rightarrow> pre_I7 ms t
-\<comment>\<open>|  fence \<Rightarrow> pre_fence ms t\<close>
-|  I8 \<Rightarrow> pre_I8 ms t
-|  I9 \<Rightarrow> pre_I9 ms t
-|  I10 \<Rightarrow> pre_I10 ms t
-|  I11 \<Rightarrow> pre_I11 ms t
-|  cas_res \<Rightarrow> pre_cas_res ms t
-|  I12 \<Rightarrow> pre_I12 ms t
-|  I13 \<Rightarrow> pre_I13 ms t
-|  I14 \<Rightarrow> pre_I14 ms t
-|  finished \<Rightarrow> True
-
-|  R1 \<Rightarrow> pre_R1 ms t
-|  R2 \<Rightarrow> pre_R2 ms t
-|  R3 \<Rightarrow> pre_R3 ms t
-|  R4 \<Rightarrow> pre_R4 ms t
-|  R5 \<Rightarrow> pre_R5 ms t
-
-|  S1 \<Rightarrow> pre_S1 ms t
-|  S2 \<Rightarrow> pre_S2 ms t
-|  S3 \<Rightarrow> pre_S3 ms t
-|  S4 \<Rightarrow> pre_S4 ms t
-|  S5 \<Rightarrow> pre_S5 ms t
-|  S6 \<Rightarrow> pre_S6 ms t
-|  S7 \<Rightarrow> pre_S7 ms t
-
-"
-
-lemmas pre_conds [simp] = pre_I1_def pre_I2_def pre_I3_def pre_I4_def pre_I5_def
-                   pre_I6_def pre_I7_def pre_I8_def pre_I9_def pre_I10_def
-                   pre_I11_def pre_I12_def pre_I13_def pre_I14_def 
-                   pre_cas_res_def 
-                   pre_R1_def pre_R2_def pre_R3_def pre_R4_def pre_R5_def
-                   pre_S1_def pre_S2_def pre_S3_def pre_S4_def pre_S5_def 
-                   pre_S6_def pre_S7_def 
-
-
-
-
-(*
-@I5 .. I11 \<forall>t'. t \<noteq> t' \<longrightarrow> t'\<notin>ownR ps n
 *)
 
-definition "init ms ps \<equiv>  (\<forall>t. (t<T_max)\<longrightarrow> pc ms t = I1
-                         \<and> n_dec ms t = False
-                         \<and> s_dec ms t = False
-                         \<and> v ms t = None
-                         \<and> n ms t = None
-                         \<and> det ms t = []
-                         \<and> CTRsync\<^sub>1 ms t = 0
-                         \<and> CTRsync\<^sub>2 ms t = 0
-                         \<and> res ms t = 0
-                         \<and> reg ms t = 0
-                         \<and> nondet_val ms t = False
-                         \<and> CAS_succ ms t = False
-                         \<and> repeat ms t = False)
-                         \<and> (\<forall>t k. (t<T_max \<and> k<T_max) \<longrightarrow> 
-                                          r ms t k = 0)
-        \<and> (\<forall>i. (i\<ge>0) \<longrightarrow> A ps i = None \<and> own\<^sub>R ms i = {} \<and> own\<^sub>W ms i = None)
-        \<and> alloc_addrs ps = {}"
-
-(* Global invariant = some general properties + what do we want to guarantee?*)
-
-(* Preconditions (local invariant) = pc = ... \<longrightarrow> P *)
 
 
-(* old main invariant version
-definition "main_invariant_1 ms \<equiv> \<forall>k t t'. ( k<length (det ms t) \<and> t'\<noteq>t \<and> t'<CTRsync\<^sub>1 ms t \<and> (r ms t t') = 0)
-                                           \<longrightarrow> t' \<notin> own\<^sub>R ms ((det ms t) ! k)"
+(*the following describes originally reserved addresses*)
+definition "default_locs \<equiv> {i | i a. i=C \<or> i = rcu_0+a \<and> a\<le>T_max }"
 
-definition "main_invariant_2 ms \<equiv> \<forall>k t t'. ( k<length (det ms t) \<and> t'\<noteq>t \<and> t'<CTRsync\<^sub>2 ms t)
-                                           \<longrightarrow> t' \<notin> own\<^sub>R ms ((det ms t) ! k)"
+definition "reserved_bydef ps \<equiv> \<forall>i. i\<in>default_locs \<longrightarrow> \<not>isfree_addr i ps"
 
-definition "main_invariant_3 ms \<sigma> \<equiv> \<forall>k t t'. ( k<length (det ms t) \<and> t'\<noteq>t \<and> CTRsync\<^sub>2 ms t < T_max 
-                                                 \<and> t'=CTRsync\<^sub>2 ms t \<and> [(rcu_0+t') \<approx>\<^sub>t 0] \<sigma>)
-                                           \<longrightarrow> t' \<notin> own\<^sub>R ms ((det ms t) ! k)"
-*)
+definition "reservations_differ \<equiv> \<forall>i. i\<le>T_max \<longrightarrow> C\<noteq>rcu_0+i"
 
-(* Main Invariant *)
-definition "main_inv ms \<equiv>\<forall>t. (t\<le>T_max 
-                            \<and> n_dec ms t = True
-                            \<and> n ms t \<noteq> None)
-                  \<longrightarrow> own\<^sub>R ms (the (n ms t)) = {t}"
+definition "con_assms ps \<equiv> reserved_bydef ps \<and> reservations_differ  "
 
-definition "main_inv_2 ms ps\<equiv> \<forall>loc. isfree_addr loc ps \<longrightarrow> own\<^sub>R ms loc = {}"
-definition "main_inv_3 ms ps\<equiv> \<forall>loc t. t\<notin>own\<^sub>R ms loc \<longrightarrow> own\<^sub>W ms loc \<noteq> Some t"
+lemmas con_lemmas [simp] = reserved_bydef_def reservations_differ_def default_locs_def
 
 
 
-lemma "main_inv_2 ms ps \<Longrightarrow> main_inv_3 ms ps \<Longrightarrow> isfree_addr loc ps \<Longrightarrow>
-          own\<^sub>R ms loc = {} \<Longrightarrow> own\<^sub>W ms loc = None"
-  apply (simp add:main_inv_2_def main_inv_3_def) 
-  by (metis empty_iff option.exhaust)
+(*----------------Main Invariant Shown--------------------*)
+
+lemma main_invariant_1_preservation:
+  "main_inv ms ps \<Longrightarrow> 
+  t\<le>T_max \<Longrightarrow>
+  general_structure ms \<Longrightarrow>
+  step ms ps \<sigma> (pc ms t) t ms' ps' \<sigma>' \<Longrightarrow> 
+  preCond ms ps \<sigma> (pc ms t) t \<Longrightarrow> 
+  cvd[C,vala] \<sigma> \<Longrightarrow>
+  observation_inv_sig ms ps \<sigma> \<Longrightarrow>
+  psem_rules ps \<Longrightarrow>
+  own\<^sub>W_n_by_t_imp ms \<Longrightarrow>
+    main_inv_1 ms'"
+  apply simp 
+  apply(simp add: step_def preCond_def general_structure_lemmas main_inv_lemmas)
+  apply(case_tac "pc ms t", simp_all add:abbr) apply clarsimp
+  apply (metis insert_not_empty option.sel) apply clarsimp
+  apply(case_tac "repeat ms t", simp_all) 
+  apply (metis option.sel)
+  apply (metis option.sel)
+  (*FAAZ*) defer
+  apply clarsimp
+  apply (metis option.sel)
+  apply clarsimp
+  apply(case_tac "snd (CAS t (a, b) ya y \<sigma> ts')", simp_all)
+  apply (metis option.sel)
+  apply (metis option.sel)
+  apply (metis Diff_empty Diff_insert0 insert_Diff singleton_insert_inj_eq)
+  apply(case_tac "CAS_succ ms t", simp_all add:abbr)
+  apply clarsimp
+  apply (metis option.sel)
+  apply(case_tac "nondet_val ms t", simp_all add:abbr)
+  apply(case_tac "det ms t \<noteq> []", simp_all add:abbr)
+  apply (metis Diff_empty Diff_insert0 insert_absorb insert_iff)
+  apply(case_tac "CTRsync\<^sub>1 ms t < T_max", simp_all add:abbr)
+  apply clarsimp
+  apply (metis option.sel)
+  apply(case_tac "CTRsync\<^sub>2 ms t < T_max", simp_all add:abbr)
+  apply(case_tac "r ms t (CTRsync\<^sub>2 ms t) = 0", simp_all add:abbr)
+  apply clarsimp
+  apply (metis option.sel)
+  apply(case_tac "reg ms t = 1", simp_all add:abbr)
+  apply(simp add: FAAZ_def get_C_val_def)
+  apply(clarsimp)  (*y \<noteq> value \<sigma> (a, b), where value \<sigma> (a, b) is retrieved from reading C*)
+  apply(simp_all add: covered_v_def lastWr_def observation_inv_sig_def visible_writes_def)
+  by (metis option.sel own\<^sub>W_n_by_t_imp_def)
+
+
+lemma main_invariant_2_preservation:
+  "main_inv ms ps \<Longrightarrow> 
+  t\<le>T_max \<Longrightarrow>
+  general_structure ms \<Longrightarrow>
+  step ms ps \<sigma> (pc ms t) t ms' ps' \<sigma>' \<Longrightarrow> 
+  preCond ms ps \<sigma> (pc ms t) t \<Longrightarrow> 
+  observation_inv_sig ms ps \<sigma> \<Longrightarrow>
+  cvd[C,vala] \<sigma> \<Longrightarrow>
+  psem_rules ps \<Longrightarrow>
+  own\<^sub>W_n_by_t_imp ms \<Longrightarrow>
+    main_inv_2 ms' ps'"
+  apply simp 
+  apply(simp add: step_def preCond_def general_structure_lemmas main_inv_lemmas)
+  apply(case_tac "pc ms t", simp_all add:abbr)
+  apply clarsimp
+  apply clarsimp
+  apply(case_tac "repeat ms t", simp_all)  
+  apply (metis subset_singleton_iff) 
+  (*FAAZ*) defer
+  apply clarsimp
+  apply clarsimp apply(case_tac " snd (CAS t (a, b) ya y \<sigma> ts')", simp_all)
+  apply(case_tac "CAS_succ ms t", simp_all add:abbr)
+  apply clarsimp
+  apply(case_tac "nondet_val ms t", simp_all add:abbr)
+  apply(case_tac "det ms t \<noteq> []", simp_all add:abbr) 
+  (*detached rules*) defer
+  apply(case_tac "CTRsync\<^sub>1 ms t < T_max", simp_all add:abbr)
+  apply clarsimp
+  apply(case_tac "CTRsync\<^sub>2 ms t < T_max", simp_all add:abbr)
+  apply(case_tac "r ms t (CTRsync\<^sub>2 ms t) = 0", simp_all add:abbr)
+  apply clarsimp
+  apply(case_tac "reg ms t = 1", simp_all add:abbr)
+  apply(simp add: FAAZ_def get_C_val_def)
+  apply(clarsimp)  (*y \<noteq> value \<sigma> (a, b), where value \<sigma> (a, b) is retrieved from reading C*)
+  apply(simp add: covered_v_def observation_inv_sig_def visible_writes_def)
+  apply blast
+  (*the detached list property*)
+  apply clarify apply(intro conjI impI)
+  apply(subgoal_tac "hd(det ms t) \<in> detaddrs ms t", simp_all) 
+  apply(subgoal_tac "det ms t \<noteq> []") prefer 2
+  apply blast
+  apply(subgoal_tac "det ms t!0 = hd(det ms t)") prefer 2
+  apply (metis hd_conv_nth)
+  by blast
 
 
 
-definition "observation_lemma_ms ms ps \<equiv> \<forall>t loc .( (t\<le>T_max \<and> the(own\<^sub>W ms (loc)) = t)) \<longrightarrow>
-                              (loc \<in> (detaddrs ms t \<union> s_and_n ms t))"
-
-definition "observation_lemma_sig ms ps \<sigma> \<equiv> \<forall>t loc .( (t\<le>T_max \<and> the(own\<^sub>W ms (loc)) = t)
-                                                      \<or> \<not>isfree_addr loc ps) \<longrightarrow>
-                               (\<exists>val . cvd[C, val] \<sigma> \<longrightarrow> val \<noteq> loc)"
-
-                                              
-lemmas new_main_inv [simp] = main_inv_def main_inv_2_def main_inv_3_def
-
-(*supporting structure invariants*)
-definition "allocated_s_addr ms ps \<equiv> \<forall>t. (t\<le>T_max \<and> (s ms t)\<noteq>None \<and> t\<in>own\<^sub>R ms (the(s ms t)))\<longrightarrow> \<not>(isfree_addr (the(s ms t)) ps)"
-definition "allocated_n_addr ms ps \<equiv> \<forall>t. (t\<le>T_max \<and> (n ms t)\<noteq>None \<and> (n_dec ms t))\<longrightarrow> \<not>(isfree_addr (the(n ms t)) ps)"
-definition "allocated_det_addr ms ps \<equiv> \<forall>t i. (t\<le>T_max \<and> det ms t\<noteq>[] \<and> i<length(det ms t))\<longrightarrow> \<not>(isfree_addr (det ms t ! i) ps)"
-
-definition "allocated_rcuandC_addr ms ps \<equiv> (\<not>(isfree_addr (C) ps)) \<and> (\<forall>i. i<T_max \<longrightarrow> \<not>(isfree_addr (rcu_0+i) ps))"
-
-definition "allocated_addresses ms ps \<equiv> allocated_s_addr ms ps \<and> allocated_n_addr ms ps \<and> 
-                                        allocated_det_addr ms ps \<and> allocated_rcuandC_addr ms ps"
-lemmas allocation_lemmas = allocated_addresses_def
-                           allocated_s_addr_def allocated_n_addr_def
-                           allocated_det_addr_def allocated_rcuandC_addr_def
-
-definition "n_is_a_unique_loc ms \<equiv> \<forall>t ta. (t\<le>T_max \<and> ta\<le>T_max \<and> ta\<noteq>t
-                                        \<and> n_dec ms t \<and> n ms t \<noteq> None) 
-                      \<longrightarrow> the(n ms t) \<notin> ({the(s ms ta),the(n ms ta)}\<union>detaddrs ms ta)"
-
-definition "n_is_a_unique_local_loc ms \<equiv> \<forall>t. (t\<le>T_max \<and> n_dec ms t \<and> n ms t \<noteq> None) 
-                      \<longrightarrow> the(n ms t) \<notin> ({the(s ms t)}\<union>detaddrs ms t)"
-
-definition "n_uniqueness ms \<equiv> n_is_a_unique_loc ms \<and> n_is_a_unique_local_loc ms"
-
-definition "s_loc_rule ms \<equiv> \<forall>t ta. (t\<le>T_max \<and> ta\<le>T_max 
-                                        \<and> s ms t \<noteq> None \<and> t\<in> own\<^sub>R ms (the(s ms t)))
-                      \<longrightarrow> the(s ms t) \<notin> (detaddrs ms ta)"
-
-
-definition "general_structure ms \<equiv> n_uniqueness ms \<and> s_loc_rule ms"
-                                       
-lemmas general_structure_lemmas = general_structure_def
-                                  n_uniqueness_def s_loc_rule_def
-                                  n_is_a_unique_loc_def n_is_a_unique_local_loc_def
-
-lemma s_allocs_differs_from_n_allocs:
-  " general_structure ms\<Longrightarrow> 
-(t\<le>T_max \<and> ta\<le>T_max\<and> n_dec ms ta \<and> n ms ta \<noteq> None) \<Longrightarrow>
-                      the(s ms t) \<noteq> the(n ms ta) "
-  apply (simp_all add:general_structure_lemmas) 
-  by metis
+lemma main_invariant_3_preservation:
+  "main_inv ms ps \<Longrightarrow> 
+  t\<le>T_max \<Longrightarrow>
+  general_structure ms \<Longrightarrow>
+  step ms ps \<sigma> (pc ms t) t ms' ps' \<sigma>' \<Longrightarrow> 
+  preCond ms ps \<sigma> (pc ms t) t \<Longrightarrow> 
+  observation_inv_sig ms ps \<sigma> \<Longrightarrow>
+  psem_rules ps \<Longrightarrow>
+  cvd[C,vala] \<sigma> \<Longrightarrow>
+  own\<^sub>W_n_by_t_imp ms \<Longrightarrow>
+    main_inv_3 ms' ps'"
+  apply simp 
+  apply(simp add: step_def preCond_def general_structure_lemmas main_inv_lemmas)
+  apply(case_tac "pc ms t", simp_all add:abbr Wcap_def Rcap_def)
+  apply clarsimp 
+  apply (meson own\<^sub>W_n_by_t_imp_def)
+  apply clarsimp
+  apply(case_tac "repeat ms t", simp_all add:own\<^sub>W_n_by_t_imp_def) 
+  apply clarsimp 
+  apply(case_tac "loc = ya", simp_all) 
+  apply (metis less_nat_zero_code list.size(3) option.sel) 
+  (*FAAZ*) defer
+  apply clarsimp apply clarsimp
+  apply(case_tac "snd (CAS t (a, b) ya y \<sigma> ts')", simp_all) 
+  apply (meson option.distinct(1)) 
+  apply (metis option.discI)
+  apply(case_tac "CAS_succ ms t", simp_all add:abbr)
+  apply clarsimp
+  apply(case_tac "nondet_val ms t", simp_all add:abbr)
+  apply(case_tac "det ms t \<noteq> []", simp_all add:abbr)
+  apply(case_tac "CTRsync\<^sub>1 ms t < T_max", simp_all add:abbr)
+  apply clarsimp
+  apply(case_tac "CTRsync\<^sub>2 ms t < T_max", simp_all add:abbr)
+  apply(case_tac "r ms t (CTRsync\<^sub>2 ms t) = 0", simp_all add:abbr)
+  apply clarsimp
+  apply(case_tac "reg ms t = 1", simp_all add:abbr)
+  apply(simp add: FAAZ_def get_C_val_def)
+  apply(clarsimp) (*y \<noteq> value \<sigma> (a, b), where value \<sigma> (a, b) is retrieved from reading C*)
+  by(case_tac "loc = value \<sigma> (a, b)", simp_all) 
 
 
 
 
+lemma main_invariant_preservation:
+  "main_inv ms ps \<Longrightarrow> 
+  t\<le>T_max \<Longrightarrow>
+  general_structure ms \<Longrightarrow>
+  step ms ps \<sigma> (pc ms t) t ms' ps' \<sigma>' \<Longrightarrow> 
+  preCond ms ps \<sigma> (pc ms t) t \<Longrightarrow> 
+  observation_inv_sig ms ps \<sigma> \<Longrightarrow>
+  cvd[C,vala] \<sigma> \<Longrightarrow>
+  psem_rules ps \<Longrightarrow>
+  own\<^sub>W_n_by_t_imp ms  \<Longrightarrow> 
+main_inv ms' ps'"
+  unfolding main_inv_def
+  apply(intro conjI impI)
+  using main_invariant_1_preservation main_inv_def apply blast
+  using main_invariant_2_preservation main_inv_def apply blast
+  using main_invariant_3_preservation main_inv_def apply blast
+  done
 
-lemma differences:
-  assumes "s ms 0 = Some 5"
-  and "s ms 1 = Some 4" 
-  and "T_max = 1"
-shows "s ms 0 \<noteq> s ms 1"
-  using assms
-  by auto
+(*--------------------------------------------------------------------*)
+
+(*------------------------Local Correctness---------------------------*)
 
 
-lemmas allocated [simp] = allocated_n_addr_def
+lemma Local_correctness:
+  "main_inv ms ps \<Longrightarrow> 
+  t\<le>T_max \<Longrightarrow>
+  general_structure ms \<Longrightarrow>
+  step ms ps \<sigma> (pc ms t) t ms' ps' \<sigma>' \<Longrightarrow> 
+  preCond ms ps \<sigma> (pc ms t) t \<Longrightarrow> 
+  observation_inv_sig ms ps \<sigma> \<Longrightarrow>
+  cvd[C,vala] \<sigma> \<Longrightarrow>
+  psem_rules ps \<Longrightarrow>
+  own\<^sub>W_n_by_t_imp ms  \<Longrightarrow> 
+preCond ms' ps' \<sigma>' (pc ms' t) t"
+  apply(simp add:preCond_def)
+  apply(simp add:step_def)
+  apply(case_tac "pc ms t", simp_all add:abbr)
+  apply(simp_all add:own\<^sub>W_n_by_t_imp_def main_inv_lemmas general_structure_lemmas)
+  apply(simp_all add:allocated_addresses_lemmas Rcap_def Wcap_def)
+  apply clarsimp
+  apply clarsimp
+  apply clarsimp
+  apply metis
+  apply metis
+  apply(case_tac "\<not>repeat ms t", simp_all)
+  apply(simp_all add:allocated_addresses_lemmas Rcap_def Wcap_def)
+  apply metis
+  apply (metis less_nat_zero_code list.size(3))
+  apply metis
+  (*FAAZ*) defer
+  apply(clarsimp)
+  apply(simp_all add:allocated_addresses_lemmas Rcap_def Wcap_def)
+  apply clarsimp
+  apply(case_tac "\<not>snd (CAS t (a, b) (the (s ms t)) (the (n ms t)) \<sigma> ts')", simp_all)
+  apply(simp add:observation_inv_sig_def covered_v_def visible_writes_def)
+  unfolding lastWr_def apply clarsimp
+  apply(simp add:allocated_addresses_lemmas Rcap_def Wcap_def)
+  apply(simp add:observation_inv_sig_def covered_v_def visible_writes_def)
+  unfolding lastWr_def apply clarsimp
+  apply(simp add:allocated_addresses_lemmas Rcap_def Wcap_def) 
+  apply clarify apply(intro conjI impI)
+  apply metis apply clarsimp
+  apply(subgoal_tac "the(n ms t) \<notin> detaddrs ms t") 
+  apply (metis detaddrs_def inlist_def mem_Collect_eq) prefer 2
+  apply(subgoal_tac "the(n ms t) \<notin> detaddrs ms t") 
+  sledgehammer
 
-lemma ms_observation_lemma_Correctness_supp_1:
+
+
+
+
+
+
+
+
+
+
+
+
+
+
+
+
+
+
+
+
+
+
+
+
+
+
+(*--------------------------------------------------------------------*)
+
+
+lemma preservation_of_variables_1_by_others:
   assumes "preCond ms ps \<sigma> (pc ms t) t"
   and "t \<le> T_max"
   and "ta \<le> T_max"
@@ -1049,14 +289,12 @@ shows "n ms ta = n ms' ta"
   apply(case_tac "pc ms t", simp_all)
   apply(simp_all add:abbr)
   apply clarify
-  apply(simp_all add:general_structure_lemmas) apply(simp add:get_C_val_def)
+  apply(simp_all add:general_structure_lemmas) apply clarsimp  apply(simp add:get_C_val_def)
   apply(simp add:FAAZ_def)
-  apply(simp add: visible_writes_def) 
-  apply(subgoal_tac "n ms t \<noteq> n ms ta") prefer 2 
-  apply metis
+  apply(simp add: visible_writes_def)
   apply clarsimp
-  apply(clarsimp)
-  apply clarify
+  apply clarsimp 
+  apply clarsimp
   apply(case_tac "snd (CAS t (a, b) (the (s ms t)) (the (n ms t)) \<sigma> ts')", simp_all)
   apply(case_tac "CAS_succ ms t", simp_all add:abbr)
   apply(clarsimp)
@@ -1069,8 +307,7 @@ shows "n ms ta = n ms' ta"
   apply(clarsimp)
   by(case_tac "reg ms t = Suc 0", simp_all add:abbr)
 
-
-lemma ms_observation_lemma_Correctness_supp_2:
+lemma preservation_of_variables_2_by_others:
   assumes "preCond ms ps \<sigma> (pc ms t) t"
   and "t \<le> T_max"
   and "ta \<le> T_max"
@@ -1087,11 +324,9 @@ shows "s ms ta = s ms' ta"
   apply(simp_all add:general_structure_lemmas)apply(simp add:get_C_val_def)
   apply(simp add:FAAZ_def)
   apply(simp add: visible_writes_def) 
-  apply(subgoal_tac "n ms t \<noteq> n ms ta") prefer 2 
-  apply metis
   apply clarsimp
-  apply(clarsimp)
-  apply clarify
+  apply clarsimp
+  apply clarsimp
   apply(case_tac "snd (CAS t (a, b) (the (s ms t)) (the (n ms t)) \<sigma> ts')", simp_all)
   apply(case_tac "CAS_succ ms t", simp_all add:abbr)
   apply(clarsimp)
@@ -1104,7 +339,7 @@ shows "s ms ta = s ms' ta"
   apply(clarsimp)
   by(case_tac "reg ms t = Suc 0", simp_all add:abbr)
 
-lemma ms_observation_lemma_Correctness_supp_3:
+lemma preservation_of_variables_3_by_others:
   assumes "preCond ms ps \<sigma> (pc ms t) t"
   and "t \<le> T_max"
   and "ta \<le> T_max"
@@ -1121,11 +356,9 @@ shows "det ms ta = det ms' ta"
   apply(simp_all add:general_structure_lemmas)apply(simp add:get_C_val_def)
   apply(simp add:FAAZ_def)
   apply(simp add: visible_writes_def) 
-  apply(subgoal_tac "n ms t \<noteq> n ms ta") prefer 2 
-  apply metis
   apply clarsimp
-  apply(clarsimp)
-  apply clarify
+  apply clarsimp
+  apply clarsimp
   apply(case_tac "snd (CAS t (a, b) (the (s ms t)) (the (n ms t)) \<sigma> ts')", simp_all)
   apply(case_tac "CAS_succ ms t", simp_all add:abbr)
   apply(clarsimp)
@@ -1137,115 +370,163 @@ shows "det ms ta = det ms' ta"
   apply(case_tac "r ms t (CTRsync\<^sub>2 ms t) = 0", simp_all add:abbr)
   apply(clarsimp)
   by(case_tac "reg ms t = Suc 0", simp_all add:abbr)
-
-lemma "\<exists>a b. A ps prov = Some (a, b) \<Longrightarrow>prov \<in> dom(A ps)"
-  by (simp add: domIff)
-
-
-
-
-
-lemma ms_observation_lemma_Correctness_supp_4:
+lemma preservation_of_variables_inset_by_others:
   assumes "preCond ms ps \<sigma> (pc ms t) t"
   and "t \<le> T_max"
+  and "ta \<noteq> t"
   and "ta \<le> T_max"
   and "step ms ps \<sigma> (pc ms t) t ms' ps' \<sigma>'"    
   and "general_structure ms"
-  and "ta \<noteq> t" 
-  and "the (own\<^sub>W ms loc) = ta"
-  and "\<not>isfree_addr loc ps"
-  and "loc \<noteq> hd (det ms t)"
-shows "the (own\<^sub>W ms' loc) = ta"
-  using assms apply (simp_all)
+  and "own\<^sub>W ms loc = Some ta"
+  and "observation_inv_ms ms"
+shows "(loc \<in> (detaddrs ms' ta) \<or> Some loc = s ms' ta \<or> Some loc = n ms' ta)"
+  using assms 
+  apply(subgoal_tac "(det ms' ta) = (det ms ta)") prefer 2 
+  using preservation_of_variables_3_by_others
+  apply force
+  apply(subgoal_tac "the (s ms' ta) = the (s ms ta)") prefer 2 
+  using preservation_of_variables_2_by_others
+  apply force
+  apply(subgoal_tac "the (n ms' ta) = the (n ms ta)") prefer 2 
+  using preservation_of_variables_1_by_others
+  apply force 
+  apply(simp add:observation_inv_ms_def) 
+  by (metis assms(5) preservation_of_variables_1_by_others preservation_of_variables_2_by_others)+
+  
+
+
+
+
+lemma preservation_of_variables_ninset_by_others:
+  assumes "preCond ms ps \<sigma> (pc ms t) t"
+  and "t \<le> T_max"
+  and "ta \<noteq> t"
+  and "ta \<le> T_max"
+  and "step ms ps \<sigma> (pc ms t) t ms' ps' \<sigma>'"    
+  and "general_structure ms"
+  and "(loc \<notin> (detaddrs ms ta) \<and> Some loc \<noteq> s ms ta \<and> Some loc \<noteq> n ms ta)"
+  and "observation_inv_ms ms"
+shows "(loc \<notin> (detaddrs ms' ta) \<and> Some loc \<noteq> s ms' ta \<and> Some loc \<noteq> n ms' ta)"
+  using assms apply simp
+  by (simp add: preservation_of_variables_1_by_others 
+                preservation_of_variables_2_by_others 
+                preservation_of_variables_3_by_others)
+lemma preservation_of_ownership_by_others:
+  "preCond ms ps \<sigma> (pc ms t) t
+\<Longrightarrow> own\<^sub>W ms loc = Some ta 
+\<Longrightarrow> ta\<noteq>t 
+\<Longrightarrow> ta\<le>T_max
+\<Longrightarrow> t\<le>T_max
+\<Longrightarrow> main_inv_2 ms ps
+\<Longrightarrow> main_inv_3 ms ps
+\<Longrightarrow> observation_inv_ms ms
+\<Longrightarrow> own\<^sub>W_n_by_t_imp ms
+\<Longrightarrow> general_structure ms
+\<Longrightarrow> step ms ps \<sigma> (pc ms t) t ms' ps' \<sigma>' 
+     \<Longrightarrow> own\<^sub>W ms' loc = Some ta"
   apply(simp add:step_def)
-  apply(simp add:preCond_def)
-  apply(case_tac "pc ms t", simp_all)
-  apply(simp_all add:abbr)
-  apply clarify
-  apply(simp_all add:general_structure_lemmas)
-  apply(subgoal_tac "loc\<noteq>loca", simp_all add:Rcap_def Wcap_def)  apply clarsimp apply(simp add:get_C_val_def)     
-  apply(simp add:FAAZ_def)
-  apply(simp add: visible_writes_def)  apply clarsimp 
-  apply clarsimp 
-  apply(simp add: visible_writes_def)   apply clarsimp
-  apply(case_tac "(snd (CAS t (a, b) (the (s ms t)) (the (n ms t)) \<sigma> ts'))", simp_all)
-  apply metis
-  apply(case_tac "CAS_succ ms t", simp_all add:abbr) apply clarsimp
-  apply(case_tac "nondet_val ms t", simp_all add:abbr) apply clarsimp
-  apply(case_tac "det ms t", simp_all add:abbr)apply clarify
-  apply(case_tac "CTRsync\<^sub>1 ms t < T_max", simp_all add:abbr) apply clarify
-  apply(case_tac "x = 0", simp_all)
+  apply(case_tac "pc ms t", simp_all add:abbr)
+  (*n:=newint*) defer
+  (*FAAZ*) defer
+  apply force
+  (*cas_step_rcu*) defer
+  apply(case_tac "CAS_succ ms t", simp_all add:abbr)
+  apply force
+  apply(case_tac "nondet_val ms t", simp_all add:abbr)
+  apply(case_tac "det ms t", simp_all add:abbr)
+  (*kill*) defer
+  apply(case_tac "CTRsync\<^sub>1 ms t < T_max", simp_all add:abbr)
+  apply force
   apply(case_tac "CTRsync\<^sub>2 ms t < T_max", simp_all add:abbr)
-  apply(case_tac "r ms t (CTRsync\<^sub>2 ms t) = 0", simp_all add:abbr) apply clarify
-  apply(case_tac "v = 0", simp_all)
-  by(case_tac "reg ms t = 1", simp_all add:abbr)
-
-
-
-
-lemma ms_observation_lemma_Correctness:
-  assumes "preCond ms ps \<sigma> pcr t"
-  and "t \<le> T_max"
-  and "main_inv ms"
-  and "main_inv_2 ms ps"
-  and "main_inv_3 ms ps"
-  and "pcr = pc ms t"
-  and "step ms ps \<sigma> pcr t ms' ps' \<sigma>'"    
-  and "general_structure ms"
-  and "pcr' = pc ms' t"
-  and "ta \<le> T_max \<and> the (own\<^sub>W ms loc) = ta"
-  and "observation_lemma_ms ms ps"
-  and "ta \<noteq> t"
-shows "loc \<in> (detaddrs ms' ta \<union> s_and_n ms' ta)"
-  using assms 
-  apply(subgoal_tac "(det ms' ta) = (det ms ta)") prefer 2 
-  using ms_observation_lemma_Correctness_supp_3 
+  apply(case_tac "r ms t (CTRsync\<^sub>2 ms t) = 0", simp_all add:abbr)
   apply force
-  apply(subgoal_tac "the (s ms' ta) = the (s ms ta)") prefer 2 
-  using ms_observation_lemma_Correctness_supp_2 
-  apply force
-  apply(subgoal_tac "the (n ms' ta) = the (n ms ta)") prefer 2 
-  using ms_observation_lemma_Correctness_supp_1
-  apply force
-  apply(simp add:observation_lemma_ms_def)
-  by meson
-
-
-lemma ms_observation_lemma_Correctness_2:
-  assumes "preCond ms ps \<sigma> pcr t"
-  and "t \<le> T_max"
-  and "main_inv ms"
-  and "main_inv_2 ms ps"
-  and "main_inv_3 ms ps"
-  and "pcr = pc ms t"
-  and "step ms ps \<sigma> pcr t ms' ps' \<sigma>'"    
-  and "general_structure ms"
-  and "pcr' = pc ms' t"
-  and "ta \<le> T_max \<and> the (own\<^sub>W ms loc) = ta"
-  and "observation_lemma_ms ms ps"
-  and "ta \<noteq> t"
-  and "\<not>isfree_addr loc ps"
-  and "loc \<noteq> hd (det ms t)"
-shows "observation_lemma_ms ms' ps'"
-  using assms 
-  apply(subgoal_tac "(det ms' ta) = (det ms ta)") prefer 2 
-  using ms_observation_lemma_Correctness_supp_3 
-  apply force
-  apply(subgoal_tac "the (s ms' ta) = the (s ms ta)") prefer 2 
-  using ms_observation_lemma_Correctness_supp_2 
-  apply force
-  apply(subgoal_tac "the (n ms' ta) = the (n ms ta)") prefer 2 
-  using ms_observation_lemma_Correctness_supp_1
-  apply force
-  apply(case_tac "the (own\<^sub>W ms loc) = ta") prefer 2
-  apply linarith 
-  apply(subgoal_tac "the (own\<^sub>W ms' loc) = ta") prefer 2 
-  using ms_observation_lemma_Correctness_supp_4 
+  apply(case_tac "reg ms t = Suc 0", simp_all add:abbr)
+  apply clarsimp
+  apply(case_tac "loc = loca", simp_all)
+  using get_C_val_def mstate.simps(17) apply force apply clarify
+  apply(case_tac "snd (CAS t (a, b) (the (s ms t)) (the (n ms t)) \<sigma> ts')", simp_all)
+  apply(simp add:observation_inv_ms_def)
+  apply(subgoal_tac "loc \<in> (detaddrs ms ta \<union> s_and_n ms ta)") prefer 2
+  apply(simp add:detaddrs_def s_and_n_def)
+  apply(simp add:general_structure_lemmas)
+  apply(simp add:preCond_def)
   apply meson
-  apply(subgoal_tac "loc \<in> (detaddrs ms' ta \<union> s_and_n ms' ta)") prefer 2
-  using ms_observation_lemma_Correctness apply blast
-  apply(simp add:observation_lemma_ms_def)
-  apply(simp add:observation_lemma_ms_def)
+  apply(simp add:general_structure_lemmas)
+  apply(simp add:preCond_def observation_inv_ms_def own\<^sub>W_n_by_t_imp_def)
+  apply(case_tac "Some loc = (n ms ta)") 
+  apply (metis (no_types, lifting) hd_conv_nth length_greater_0_conv option.distinct(1) option.sel)
+  apply (metis (no_types, lifting) option.sel)
+  apply(simp add:preCond_def Wcap_def) 
+  apply (metis option.sel)
+  apply(simp add:preCond_def Wcap_def) 
+  apply(simp add:general_structure_lemmas)
+  (*ta cannot own\<^sub>W ms LOC where LOC \<in> det_addrs ms t*) 
+  sorry
+  
+  
+
+lemma preservation_of_nownership_by_others:
+  "preCond ms ps \<sigma> (pc ms t) t
+\<Longrightarrow> own\<^sub>W ms loc \<noteq> Some ta 
+\<Longrightarrow> ta\<noteq>t 
+\<Longrightarrow> t\<le>T_max 
+\<Longrightarrow> ta\<le>T_max
+\<Longrightarrow> step ms ps \<sigma> (pc ms t) t ms' ps' \<sigma>' 
+     \<Longrightarrow> own\<^sub>W ms' loc \<noteq> Some ta"
+  apply (simp add:step_def)
+  apply(case_tac "pc ms t", simp_all add:abbr)
+  apply safe
+  apply (smt (z3) fun_upd_apply mstate.simps(17) mstate.surjective mstate.update_convs(1) mstate.update_convs(16) mstate.update_convs(17) option.sel)
+  apply(simp add:get_C_val_def FAAZ_def)
+  apply safe 
+  apply simp+
+  apply(case_tac "loc = the (n ms t)", simp_all)
+  apply(case_tac "CAS_succ ms t", simp_all add:abbr)
+  apply(case_tac "nondet_val ms t", simp_all add:abbr)
+  apply(case_tac "det ms t", simp_all add:abbr)
+  apply(case_tac "CTRsync\<^sub>1 ms t < T_max", simp_all add:abbr)
+  apply(case_tac "CTRsync\<^sub>2 ms t < T_max", simp_all add:abbr)
+  apply(case_tac "r ms t (CTRsync\<^sub>2 ms t) = 0", simp_all add:abbr)
+  by(case_tac "reg ms t = Suc 0", simp_all add:abbr)
+
+
+lemma preservation_of_observation_inv_ms:
+  assumes "preCond ms ps \<sigma> (pc ms t) t"
+  and "t \<le> T_max"
+  and "step ms ps \<sigma> (pc ms t) t ms' ps' \<sigma>'"    
+  and "general_structure ms"
+  and "observation_inv_ms ms"
+  and "main_inv_2 ms ps"
+  and "main_inv_3 ms ps"
+  and "observation_inv_sig ms ps \<sigma>"
+  and "own\<^sub>W_n_by_t_imp ms"
+  and "general_structure ms"
+  and "psem_rules ps"
+shows "observation_inv_ms ms'"
+  using assms unfolding observation_inv_ms_def apply simp apply clarify
+  apply(case_tac "ta \<noteq> t")
+  (*ta\<noteq>t*)
+  apply(simp add:step_def preCond_def)
+  apply(case_tac "pc ms t", simp_all add:abbr)
+  apply clarsimp 
+  apply blast
+  apply blast
+  apply blast 
+  apply clarsimp 
+  apply (meson own\<^sub>W_n_by_t_imp_def)
+  apply (meson own\<^sub>W_n_by_t_imp_def)
+  apply (meson own\<^sub>W_n_by_t_imp_def)
+  apply (meson own\<^sub>W_n_by_t_imp_def)
+  (*FAAZ, ta\<noteq>t*) defer
+  apply(simp add:Wcap_def own\<^sub>W_n_by_t_imp_def general_structure_lemmas Rcap_def)
+  sledgehammer
+
+
+
+
+
+
+
   sorry
 
 
@@ -1258,25 +539,228 @@ shows "observation_lemma_ms ms' ps'"
 
 
 
-lemma sigma_observation_lemma_Correctness:
+
+
+
+
+
+
+
+
+
+
+
+
+
+
+
+
+
+lemma own\<^sub>W_imp_not_free:
+  assumes "main_inv ms ps"
+  and "own\<^sub>W ms loc \<noteq> None"
+shows "\<not>isfree_addr loc ps"
+  using assms apply (simp_all add:main_inv_def)
+  by blast
+
+
+
+
+lemma global_sig_invariant_preserved:
+  "con_assms ps \<Longrightarrow>
+main_inv ms ps\<Longrightarrow>
+observation_inv_ms ms\<Longrightarrow>
+main_inv_2 ms ps\<Longrightarrow> 
+main_inv_3 ms ps\<Longrightarrow> 
+observation_inv_sig ms ps \<sigma>\<Longrightarrow> 
+own\<^sub>W_n_by_t_imp ms\<Longrightarrow> 
+general_structure ms\<Longrightarrow> 
+psem_rules ps\<Longrightarrow> 
+t \<le> T_max\<Longrightarrow>
+step ms ps \<sigma> (pc ms t) t ms' ps' \<sigma>'\<Longrightarrow>
+preCond ms ps \<sigma> (pc ms t) t\<Longrightarrow>
+observation_inv_sig ms' ps' \<sigma>'
+"
+  unfolding observation_inv_sig_def step_def preCond_def
+  apply(case_tac "pc ms t", simp_all add:abbr covered_v_def con_assms_def main_inv_def observation_inv_ms_def)
+  apply(simp_all add:own\<^sub>W_n_by_t_imp_def general_structure_lemmas)
+  apply meson
+  apply meson
+  apply meson
+  apply (metis domI domIff)  apply clarsimp sledgehammer
+  apply (metis domI domIff)
+  apply (metis domI domIff)
+  apply meson
+  apply meson
+  apply meson
+
+
+
+
+
+
+
+
+
+
+
+
+lemma ms_observation_lemma_Correctness_supp_4:
   assumes "preCond ms ps \<sigma> (pc ms t) t"
-  and "wfs \<sigma>"
   and "t \<le> T_max"
+  and "ta \<le> T_max"
   and "step ms ps \<sigma> (pc ms t) t ms' ps' \<sigma>'"    
   and "general_structure ms"
-  and "observation_lemma_ms ms ps"
-  and "observation_lemma_sig ms ps \<sigma>"
+  and "ta \<noteq> t" 
+  and "own\<^sub>W ms loc = Some ta"
   and "main_inv ms"
   and "main_inv_2 ms ps"
   and "main_inv_3 ms ps"
-  and "cvd[C,vala] \<sigma>"
-shows "observation_lemma_sig ms' ps' \<sigma>'"
+  and "observation_inv_ms ms"
+shows "own\<^sub>W ms' loc = Some ta"
+  using assms 
+  apply(subgoal_tac "\<not>isfree_addr loc ps") prefer 2
+  apply (metis option.distinct(1) own_imp_1) apply (simp_all)
+  apply(simp add:step_def)
+  apply(simp add:preCond_def)
+  apply(case_tac "pc ms t", simp_all)
+  apply(simp_all add:abbr)
+  apply clarify
+  apply(simp_all add:general_structure_lemmas)
+  apply(subgoal_tac "loc\<noteq>loca", simp_all add:Rcap_def Wcap_def) 
+  apply clarsimp apply(simp add:get_C_val_def)
+  apply(simp add:FAAZ_def)
+  apply(simp add: visible_writes_def)  apply clarsimp 
+  apply clarsimp 
+  apply(simp add: visible_writes_def)   apply clarsimp
+  apply(case_tac "(snd (CAS t (a, b) (the (s ms t)) (the (n ms t)) \<sigma> ts'))", simp_all)
+  apply (metis option.sel)
+  apply(case_tac "CAS_succ ms t", simp_all add:abbr) apply clarsimp
+  apply(case_tac "nondet_val ms t", simp_all add:abbr) apply clarsimp
+  apply(case_tac "det ms t", simp_all add:abbr observation_inv_ms_def) apply clarify
+  apply clarsimp
+  sorry
+
+
+
+
+
+lemma FAAZ_wm_prelim1:
+  assumes "ms \<sigma> s:=\<^sup>FC t ms' \<sigma>'"
+  and "wfs \<sigma>"
+  and "cvd[C,valaa] \<sigma>"
+shows "cvd[C,valaa] \<sigma>'"
+  using assms apply (simp add:get_C_val_def FAAZ_def) apply(clarify) 
+  apply(simp add:update_trans_def covered_v_def Let_def rev_app_def add_cv_def update_mods_def update_modView_def
+      update_thrView_def)
+  apply(unfold writes_on_def value_def lastWr_def) apply safe
+  apply (metis fst_conv var_def)
+  apply (metis fst_conv var_def visible_var)
+  apply (metis fst_conv var_def visible_var)
+  apply (metis fst_conv var_def)
+  apply(simp add:visible_writes_def tst_def var_def valid_fresh_ts_def)
+  apply(unfold writes_on_def value_def lastWr_def wfs_def var_def) apply safe
+  (*ts; is max, nempty \<and> finite*) defer
+  apply auto[1]    
+  apply(simp) apply(intro conjI)
+  apply (meson subset_iff visible_writes_in_writes)
+  apply presburger
+  apply (metis fst_conv)
+  apply (metis fst_conv var_def visible_var)
+  apply (metis fst_conv var_def visible_var)
+  apply (metis fst_conv)
+  (*ts; is max*) defer    
+  apply(simp) apply(intro conjI)
+  apply (meson subset_iff visible_writes_in_writes)
+  apply presburger
+  sorry
+
+lemma FAAZ_wm_prelim2:
+  assumes "ms \<sigma> s:=\<^sup>FC t ms' \<sigma>'"
+  and "wfs \<sigma>"
+  and "\<exists>val. cvd[C,val] \<sigma> \<and> val\<noteq> loca"
+shows "\<exists>val. cvd[C,val] \<sigma>' \<and> val\<noteq> loca"
+  using assms
+  using FAAZ_wm_prelim1 by blast
+
+lemma FAAZ_wm_prelim3:
+  assumes "ms \<sigma> s:=\<^sup>FC t ms' \<sigma>'"
+  and "wfs \<sigma>"
+  and "cvd[C,valaa] \<sigma>"
+  and "valaa \<noteq> loca"
+shows "\<exists>val. cvd[C,val] \<sigma>' \<and> val\<noteq> loca"
+  using assms 
+  using FAAZ_wm_prelim1 by blast
+
+lemma FAAZ_wm_prelim4:
+  assumes "ms \<sigma> s:=\<^sup>FC t ms' \<sigma>'"
+  and "wfs \<sigma>"
+  and "observation_inv_sig ms ps \<sigma>"
+  and "psem_rules ps "
+  and "general_structure ms"
+shows "observation_inv_sig ms' ps' \<sigma>'"
+  using assms 
+  apply(simp add:observation_inv_sig_def general_structure_lemmas)
+  apply clarify
+  apply(intro conjI impI)
+  apply(case_tac "ta = t")
+  apply(subgoal_tac "own\<^sub>W ms loc = Some ta \<longrightarrow> own\<^sub>W ms' loc = Some ta", simp_all)
+  apply(simp add:get_C_val_def)
+  sledgehammer
+
+
+
+
+lemma sigma_observation_lemma_Correctness:
+  assumes "preCond ms ps \<sigma> (pc ms t) t"
+  and "wfs \<sigma>"
+  and "psem_rules ps"
+  and "t \<le> T_max"
+  and "step ms ps \<sigma> (pc ms t) t ms' ps' \<sigma>'"    
+  and "general_structure ms"
+  and "observation_inv_ms ms"
+  and "observation_inv_sig ms ps \<sigma>"
+  and "main_inv ms"
+  and "main_inv_2 ms ps"
+  and "main_inv_3 ms ps"
+shows "observation_inv_sig ms' ps' \<sigma>'"
   using assms apply (simp_all)
   apply(simp add:preCond_def RCU.step_def)
   apply(case_tac "pc ms t", simp_all add:abbr)
   apply(simp add:covered_v_def general_structure_lemmas )
   apply clarify
-  apply(unfold observation_lemma_sig_def observation_lemma_ms_def)
+  apply(unfold observation_inv_sig_def observation_inv_ms_def)
+  apply clarify apply(simp_all)
+  apply(case_tac "isfree_addr loc ps", simp_all)
+  apply blast apply clarify
+  apply(case_tac "isfree_addr loc ps", simp_all)
+  apply clarify
+  apply(case_tac "isfree_addr loc ps", simp_all)
+  apply clarify apply(simp add:general_structure_lemmas)
+  apply(case_tac "loc = loca", simp_all) 
+  apply metis 
+  apply meson 
+  defer (*rcu_enter*)
+  defer (*rcu_exit*)
+  defer (*rcu_enter*)
+  apply clarify
+  apply(intro conjI impI)
+  using FAAZ_wm_prelim2 [where ms = ms and ms' = ms' and \<sigma> = \<sigma> and \<sigma>' = \<sigma>' and t=t and loca=loc]
+  apply simp
+  apply(clarsimp)
+  apply(case_tac "t \<le> T_max \<and> own\<^sub>W ms loca = Some t", simp_all)
+  apply (meson FAAZ_wm_prelim1)
+  apply(case_tac "((\<forall>x. (\<forall>a. x = {a} \<longrightarrow> (\<forall>b. (a, b) \<notin> ran (A ps))) \<or> loca \<notin> x))")
+  apply (metis FAAZ_wm_prelim1)
+  apply clarify
+  sledgehammer
+
+
+  apply metis
+  apply(simp add:general_structure_lemmas)
+  sledgehammer
+
+
   by (metis (full_types))+
 
 
@@ -1284,24 +768,29 @@ shows "observation_lemma_sig ms' ps' \<sigma>'"
 lemma ms_observation_lemma_Correctnesssss:
   assumes "preCond ms ps \<sigma> (pc ms t) t"
   and "wfs \<sigma>"
+  and "psem_rules ps"
   and "t \<le> T_max"
   and "step ms ps \<sigma> (pc ms t) t ms' ps' \<sigma>'"    
   and "general_structure ms"
-  and "observation_lemma_ms ms ps"
-  and "observation_lemma_sig ms ps \<sigma>"
+  and "observation_inv_ms ms ps"
+  and "observation_inv_sig ms ps \<sigma>"
   and "main_inv ms"
   and "main_inv_2 ms ps"
   and "main_inv_3 ms ps"
   and "cvd[C,vala] \<sigma>"
-shows "observation_lemma_ms ms' ps'"
-  using assms apply (simp_all)
-  apply(simp add:preCond_def RCU.step_def)
-  apply(case_tac "pc ms t", simp_all add:abbr)
-  apply(simp add:covered_v_def general_structure_lemmas )
+shows "observation_inv_ms ms' ps'"
+  using assms apply (simp_all) 
+  apply(simp add:preCond_def)
+  apply(case_tac "pc ms t", simp_all)
+  apply(simp add:covered_v_def general_structure_lemmas)
   apply clarify
-  apply(unfold observation_lemma_sig_def observation_lemma_ms_def)
+  apply(unfold observation_inv_sig_def observation_inv_ms_def)
   apply(subgoal_tac "\<forall>loc t. t\<le>T_max \<and> own\<^sub>W ms' loc  = Some t
   \<longrightarrow> loc\<in>(detaddrs ms' t \<union> s_and_n ms' t) ") 
+  apply clarify
+  apply(subgoal_tac "loc \<in> detaddrs ms ta", simp add:detaddrs_def)
+  apply blast
+
   sorry
 
 
@@ -1323,8 +812,8 @@ lemma main_invariant_Correctness:
   and "step ms ps \<sigma> pcr t ms' ps' \<sigma>'"    
   and "general_structure ms"
   and "pcr' = pc ms' t"
-  and "observation_lemma_ms ms ps"
-  and "observation_lemma_sig ms ps \<sigma>"
+  and "observation_inv_ms ms ps"
+  and "observation_inv_sig ms ps \<sigma>"
 shows "main_inv ms'"
   using assms apply (simp add:preCond_def step_def)
   apply(case_tac[!] "pc ms t", simp_all add:abbr) 
